finished Block case for alpha equivalence step correctness

Transformations/Alpha_Equiv_Fun.thy
@@ -7,7 +7,6 @@ begin
  * based on Renamer_DeBruijn_Ext_Correct, but hopefully simpler to reason on *)
 type_synonym subst =
   "(YulIdentifier * YulIdentifier) list list"
-
 type_synonym subst' = "(YulIdentifier * YulIdentifier) list"
 
 definition subst_get1 :: "subst \<Rightarrow> YulIdentifier list list" where
@@ -37,24 +36,6 @@ definition subst_ok :: "subst \<Rightarrow> bool" where
 "subst_ok x =
   True"
 
-(*
-fun get_var_decls' ::
-  "('v, 't) YulStatement list \<Rightarrow> nat \<Rightarrow>
-   (YulIdentifier list * nat)" where
-"get_var_decls' [] i = ([], i)"
-| "get_var_decls' ((YulVariableDeclarationStatement (YulVariableDeclaration decls v))#t) i =
-   (case get_var_decls' t (i + length decls) of
-    (l', i') \<Rightarrow>
-    ((map (\<lambda> x . case x of (YulTypedName n _) \<Rightarrow> n) decls) @ l', i'))"
-| "get_var_decls' (h#t) i = get_var_decls' t i"
-
-definition get_var_decls ::
-  "('v, 't) YulStatement list \<Rightarrow> YulIdentifier list" where
-"get_var_decls l =
-  (case get_var_decls' l 0 of
-    (l', _) \<Rightarrow> l')"
-*)
-
 fun get_var_decls ::
   "('v, 't) YulStatement list \<Rightarrow>
    (YulIdentifier list)" where
@@ -62,28 +43,6 @@ fun get_var_decls ::
 | "get_var_decls ((YulVariableDeclarationStatement (YulVariableDeclaration decls v))#t) =
    (map (\<lambda> x . case x of (YulTypedName n _) \<Rightarrow> n) decls) @ (get_var_decls t)"
 | "get_var_decls (h#t) = get_var_decls t"
-
-(*
-fun get_fun_decls' ::
-"('v, 't) YulStatement list \<Rightarrow> nat \<Rightarrow>
- (YulIdentifier list * nat)" where
-"get_fun_decls' [] i = ([], i)"
-| "get_fun_decls' ((YulFunctionDefinitionStatement (YulFunctionDefinition name args rets body))#t) i =
-   (case get_fun_decls' t (i + 1) of
-     (l', i') \<Rightarrow> 
-     (name # l'
-     , i'))"
-| "get_fun_decls' (h#t) i = 
-    get_fun_decls' t i"
-
-definition get_fun_decls ::
-"('v, 't) YulStatement list \<Rightarrow>
- (YulIdentifier list)" where
-"get_fun_decls l =
-  (case get_fun_decls' l 0 of
-    (l', _) \<Rightarrow> l')"
-*)
-
 
 fun get_fun_decls ::
 "('v, 't) YulStatement list \<Rightarrow>
@@ -94,40 +53,116 @@ fun get_fun_decls ::
 | "get_fun_decls (h#t) = 
     get_fun_decls t"
 
-fun alpha_equiv_expr' ::
-  "subst \<Rightarrow> ('v, 't) YulExpression \<Rightarrow> ('v, 't) YulExpression \<Rightarrow> bool" where
-  "alpha_equiv_expr' fsubst
-    (YulLiteralExpression x1) (YulLiteralExpression x2) = (x1 = x2)"
-| "alpha_equiv_expr' fsubst
-    (YulIdentifier x1) (YulIdentifier x2) = (x1 = x2)"
-(* TODO: we may need to either put a stronger predicate on subst,
- * or have these checks go "both ways" *)
-| "alpha_equiv_expr' fsubst
-    (YulFunctionCallExpression (YulFunctionCall fn1 args1))
-    (YulFunctionCallExpression (YulFunctionCall fn2 args2)) =
-    (subst_lookup fsubst fn1 = Some fn2 \<and>
-     subst_lookup (subst_flip fsubst) fn2 = Some fn1 \<and>
-    (list_all2 (alpha_equiv_expr' fsubst) args1 args2))"
-| "alpha_equiv_expr' _ _ _ = False"
+(* whenever we extend the variable context, we also need to update subst.  *)
+(* also need to update subst on function entry. *)
 
-definition alpha_equiv_name' :: "subst \<Rightarrow> YulIdentifier \<Rightarrow> YulIdentifier \<Rightarrow> bool" where
-"alpha_equiv_name' scopes n1 n2 =
-  (subst_lookup scopes n1 = Some n2 \<and>
-   subst_lookup (subst_flip scopes) n2 = Some n1)"
+(* gather yul functions / get_fun_decls *)
 
-definition alpha_equiv_typed_name' ::
-  "subst \<Rightarrow> ('t) YulTypedName \<Rightarrow> ('t) YulTypedName \<Rightarrow> bool" where
-"alpha_equiv_typed_name' subst tn1 tn2 =
-  (case tn1 of
-    (YulTypedName n1 t1) \<Rightarrow>
-      (case tn2 of
-        (YulTypedName n2 t2) \<Rightarrow>
-          (case subst_lookup subst n1 of
-            None \<Rightarrow> False
-            | Some n2' \<Rightarrow> 
-              (case subst_lookup (subst_flip subst) n2 of
-                None \<Rightarrow> False
-                | Some n1' \<Rightarrow> t1 = t2 \<and> n1 = n1' \<and> n2 = n2'))))"
+fun subst_update_enter_statement ::
+  "subst \<Rightarrow> 
+   ('v, 't) YulStatement \<Rightarrow>
+   ('v, 't) YulStatement \<Rightarrow>
+   (subst)" where
+"subst_update_enter_statement fsubst (YulBlock ls1) (YulBlock ls2) =
+  ((zip (get_fun_decls ls1) (get_fun_decls ls2))# fsubst)"
+| "subst_update_enter_statement fsubst _ _ = (fsubst)"
+
+fun subst_update_exit_statement ::
+  "subst \<Rightarrow> 
+   ('v, 't) YulStatement \<Rightarrow>
+   ('v, 't) YulStatement \<Rightarrow>
+   (subst) option" where
+"subst_update_exit_statement fsubst
+  (YulVariableDeclarationStatement (YulVariableDeclaration ns1 eo1))
+  (YulVariableDeclarationStatement (YulVariableDeclaration ns2 eo2)) = Some fsubst"
+| "subst_update_exit_statement fsubst
+  (YulBlock ls1)
+  (YulBlock ls2) = 
+  (case (fsubst) of
+    (fsh # fsubst') \<Rightarrow> Some (fsubst')
+   | _ \<Rightarrow> None)"
+(* bogus cases mixed with noop cases here. *)
+| "subst_update_exit_statement fsubst _ _ = Some (fsubst)" 
+
+(* TODO: update fsubst with sig? *)
+fun subst_update_enter_fun_call ::
+    "subst \<Rightarrow> ('g, 'v, 't, 'z) function_sig'_scheme \<Rightarrow> ('g, 'v, 't, 'z) function_sig'_scheme \<Rightarrow> (subst)"
+    where
+  "subst_update_enter_fun_call fsubst
+    sig1 sig2 = fsubst
+    "
+
+fun subst_update_exit_fun_call ::
+  "subst \<Rightarrow>  (subst) option"
+  where
+"subst_update_exit_fun_call (fsh # fsubst') = Some (fsubst')"
+| "subst_update_exit_fun_call fsubst = None"
+
+fun subst_update ::
+  "subst \<Rightarrow> ('g, 'v, 't) StackEl \<Rightarrow> ('g, 'v, 't) StackEl \<Rightarrow> (subst) option" where
+"subst_update fsubst (EnterStatement s1) (EnterStatement s2) =
+  Some (subst_update_enter_statement fsubst s1 s2)"
+| "subst_update fsubst (ExitStatement s1 _ _) (ExitStatement s2 _ _) =
+  subst_update_exit_statement fsubst s1 s2"
+| "subst_update fsubst (EnterFunctionCall f1 s1) (EnterFunctionCall f2 s2) =
+  Some (subst_update_enter_fun_call fsubst s1 s2)"
+| "subst_update fsubst (ExitFunctionCall _ _ _ _ _) (ExitFunctionCall _ _ _ _ _) = 
+  subst_update_exit_fun_call fsubst"
+| "subst_update fsubst _ _ = Some (fsubst)"
+
+
+fun subst_updatex_enter_statement ::
+  "subst \<Rightarrow> 
+   ('v, 't) YulStatement \<Rightarrow>
+   ('v, 't) YulStatement \<Rightarrow>
+   (subst)" where
+"subst_updatex_enter_statement fsubst (YulBlock ls1) (YulBlock ls2) =
+  (fsubst)"
+| "subst_updatex_enter_statement fsubst _ _ = (fsubst)"
+
+fun subst_updatex_exit_statement ::
+  "subst \<Rightarrow> 
+   ('v, 't) YulStatement \<Rightarrow>
+   ('v, 't) YulStatement \<Rightarrow>
+   (subst) option" where
+"subst_updatex_exit_statement fsubst
+  (YulVariableDeclarationStatement (YulVariableDeclaration ns1 eo1))
+  (YulVariableDeclarationStatement (YulVariableDeclaration ns2 eo2)) = Some fsubst"
+| "subst_updatex_exit_statement fsubst
+  (YulBlock ls1)
+  (YulBlock ls2) = 
+  (case (fsubst) of
+    (fsh # fsubst') \<Rightarrow> Some (fsubst')
+   | _ \<Rightarrow> None)"
+(* bogus cases mixed with noop cases here. *)
+| "subst_updatex_exit_statement fsubst _ _ = Some (fsubst)" 
+
+(* TODO: update fsubst with sig? *)
+fun subst_updatex_enter_fun_call ::
+    "subst \<Rightarrow> ('g, 'v, 't, 'z) function_sig'_scheme \<Rightarrow> ('g, 'v, 't, 'z) function_sig'_scheme \<Rightarrow> (subst)"
+    where
+  "subst_updatex_enter_fun_call fsubst
+    sig1 sig2 = fsubst
+    "
+
+fun subst_updatex_exit_fun_call ::
+  "subst \<Rightarrow>  (subst) option"
+  where
+"subst_updatex_exit_fun_call (fsh # fsubst') = Some (fsubst')"
+| "subst_updatex_exit_fun_call fsubst = None"
+
+fun subst_updatex ::
+  "subst \<Rightarrow> ('g, 'v, 't) StackEl \<Rightarrow> ('g, 'v, 't) StackEl \<Rightarrow> (subst) option" where
+"subst_updatex fsubst (EnterStatement s1) (EnterStatement s2) =
+  Some (subst_updatex_enter_statement fsubst s1 s2)"
+| "subst_updatex fsubst (ExitStatement s1 _ _) (ExitStatement s2 _ _) =
+  subst_updatex_exit_statement fsubst s1 s2"
+| "subst_updatex fsubst (EnterFunctionCall f1 s1) (EnterFunctionCall f2 s2) =
+  Some (subst_updatex_enter_fun_call fsubst s1 s2)"
+| "subst_updatex fsubst (ExitFunctionCall _ _ _ _ _) (ExitFunctionCall _ _ _ _ _) = 
+  subst_updatex_exit_fun_call fsubst"
+| "subst_updatex fsubst _ _ = Some (fsubst)"
+
 
 (*
 definition alpha_equiv_check_decls ::
@@ -217,11 +252,59 @@ fun alpha_equiv_check_decls ::
      else None)"
 | "alpha_equiv_check_decls _ _ = None"
 
-(* bool argument is True if we are exiting statement - in these cases
- * we need to make sure we do not augment the context *)
+definition alpha_equiv_name' :: "subst \<Rightarrow> YulIdentifier \<Rightarrow> YulIdentifier \<Rightarrow> bool" where
+"alpha_equiv_name' scopes n1 n2 =
+  (subst_lookup scopes n1 = Some n2 \<and>
+   subst_lookup (subst_flip scopes) n2 = Some n1)"
+
+definition alpha_equiv_typed_name' ::
+  "subst \<Rightarrow> ('t) YulTypedName \<Rightarrow> ('t) YulTypedName \<Rightarrow> bool" where
+"alpha_equiv_typed_name' subst tn1 tn2 =
+  (case tn1 of
+    (YulTypedName n1 t1) \<Rightarrow>
+      (case tn2 of
+        (YulTypedName n2 t2) \<Rightarrow>
+          (case subst_lookup subst n1 of
+            None \<Rightarrow> False
+            | Some n2' \<Rightarrow> 
+              (case subst_lookup (subst_flip subst) n2 of
+                None \<Rightarrow> False
+                | Some n1' \<Rightarrow> t1 = t2 \<and> n1 = n1' \<and> n2 = n2'))))"
+
+definition alpha_equiv_local ::
+  "subst \<Rightarrow> (YulIdentifier * 'v) \<Rightarrow> (YulIdentifier * 'v) \<Rightarrow> bool" where
+"alpha_equiv_local fsubst loc1 loc2 =
+  (case loc1 of (n1, v1) \<Rightarrow>
+  (case loc2 of (n2, v2) \<Rightarrow>
+  (v1 = v2 \<and> n1 = n2)))"
+
+definition alpha_equiv_locals' ::
+  "subst \<Rightarrow> (YulIdentifier * 'v) list \<Rightarrow> (YulIdentifier * 'v) list \<Rightarrow> bool" where
+"alpha_equiv_locals' fsubst locs1 locs2 =
+  (locs1 = locs2)"
+
+
+fun  alpha_equiv_expr' ::
+  "subst \<Rightarrow> ('v, 't) YulExpression \<Rightarrow> ('v, 't) YulExpression \<Rightarrow> bool" where
+  "alpha_equiv_expr' fsubst
+    (YulLiteralExpression x1) (YulLiteralExpression x2) = (x1 = x2)"
+| "alpha_equiv_expr' fsubst
+    (YulIdentifier x1) (YulIdentifier x2) = (x1 = x2)"
+(* Should be sufficient to just check for a name match here*)
+| "alpha_equiv_expr' fsubst
+    (YulFunctionCallExpression (YulFunctionCall fn1 args1))
+    (YulFunctionCallExpression (YulFunctionCall fn2 args2)) =
+    (subst_lookup fsubst fn1 = Some fn2 \<and>
+     subst_lookup (subst_flip fsubst) fn2 = Some fn1 \<and>
+    (list_all2 (alpha_equiv_expr' fsubst) args1 args2))"
+| "alpha_equiv_expr' _ _ _ = False"
+
+
+
+(* TODO: get rid of bool argument, fix how we construct contexts. *)
 fun alpha_equiv_statement' ::
-  "subst \<Rightarrow> bool \<Rightarrow> ('v, 't) YulStatement \<Rightarrow> ('v, 't) YulStatement \<Rightarrow> bool" where
-  "alpha_equiv_statement' fsubst is_exit
+  "subst \<Rightarrow> ('v, 't) YulStatement \<Rightarrow> ('v, 't) YulStatement \<Rightarrow> bool" where
+  "alpha_equiv_statement' fsubst
     (YulFunctionCallStatement (YulFunctionCall fn1 args1)) stm2 =
     (case stm2 of
       (YulFunctionCallStatement (YulFunctionCall fn2 args2)) \<Rightarrow>
@@ -230,14 +313,14 @@ fun alpha_equiv_statement' ::
         (list_all2 (alpha_equiv_expr' fsubst) args1 args2))
       | _ \<Rightarrow> False)"
 
-| "alpha_equiv_statement' fsubst is_exit
+| "alpha_equiv_statement' fsubst
     (YulAssignmentStatement (YulAssignment ns1 e1)) stm2 =
     (case stm2 of
       (YulAssignmentStatement (YulAssignment ns2 e2)) \<Rightarrow>
         (alpha_equiv_expr' fsubst e1 e2 \<and> ns1 = ns2)
       | _ \<Rightarrow> False)"
 
-| "alpha_equiv_statement' fsubst is_exit
+| "alpha_equiv_statement' fsubst
     (YulVariableDeclarationStatement (YulVariableDeclaration ns1 eo1)) stm2 =
     (case stm2 of
       (YulVariableDeclarationStatement (YulVariableDeclaration ns2 eo2)) \<Rightarrow>
@@ -248,7 +331,7 @@ fun alpha_equiv_statement' ::
          (ns1 = ns2))
       | _ \<Rightarrow> False)"
 
-| "alpha_equiv_statement' fsubst is_exit
+| "alpha_equiv_statement' fsubst
   (YulFunctionDefinitionStatement
       (YulFunctionDefinition name1 args1 rets1 body1)) stm2 =
   (case stm2 of
@@ -260,12 +343,12 @@ fun alpha_equiv_statement' ::
             (args1 = args2 \<and>
              rets1 = rets2 \<and>
              (list_all2 (alpha_equiv_statement' 
-              (fsubst' # fsubst) False)
+              (fsubst' # fsubst))
               body1 body2)))
       | _ \<Rightarrow> False)"
 
 (* TODO: need entry/exit  cases? *)
-| "alpha_equiv_statement' fsubst is_exit
+| "alpha_equiv_statement' fsubst
   (YulIf e1 body1) stm2 =
   (case stm2 of
     (YulIf e2 body2) \<Rightarrow>
@@ -273,12 +356,12 @@ fun alpha_equiv_statement' ::
       (case alpha_equiv_check_decls body1 body2 of
         None \<Rightarrow> False
         | Some (fsubst') \<Rightarrow>
-          list_all2 (alpha_equiv_statement' (fsubst' # fsubst) False) body1 body2))
+          list_all2 (alpha_equiv_statement' (fsubst' # fsubst)) body1 body2))
     | _ \<Rightarrow> False)"
 
 (* TODO: need entry/exit  cases? *)
 
-| "alpha_equiv_statement' fsubst is_exit
+| "alpha_equiv_statement' fsubst
   (YulSwitch e1 cases1) stm2 =
   (case stm2 of
     (YulSwitch e2 cases2) \<Rightarrow>
@@ -293,13 +376,13 @@ fun alpha_equiv_statement' ::
             (case alpha_equiv_check_decls body1 body2 of
               None \<Rightarrow> False
               | Some (fsubst') \<Rightarrow>
-                list_all2 (alpha_equiv_statement' (fsubst' # fsubst) False) body1 body2)))))
+                list_all2 (alpha_equiv_statement' (fsubst' # fsubst)) body1 body2)))))
         cases1 cases2))
     | _ \<Rightarrow> False)"
 
 (* TODO: need entry/exit  cases? *)
 
-| "alpha_equiv_statement' fsubst is_exit
+| "alpha_equiv_statement' fsubst
   (YulForLoop pre1 cond1 post1 body1) stm2 =
   (case stm2 of
     (YulForLoop pre2 cond2 post2 body2) \<Rightarrow>
@@ -313,86 +396,42 @@ fun alpha_equiv_statement' ::
         None \<Rightarrow> False
         | Some (fsubst'_body) \<Rightarrow>
           (alpha_equiv_expr' (fsubst'_pre # fsubst) cond1 cond2 \<and>
-           list_all2 (alpha_equiv_statement' (fsubst'_pre # fsubst) False) pre1 pre2 \<and>
-           list_all2 (alpha_equiv_statement' ((fsubst'_body @ fsubst'_pre) # fsubst) False) body1 body2 \<and>
-           list_all2 (alpha_equiv_statement' ((fsubst'_post @ fsubst'_pre) # fsubst) False) post1 post2))))
+           list_all2 (alpha_equiv_statement' (fsubst'_pre # fsubst)) pre1 pre2 \<and>
+           list_all2 (alpha_equiv_statement' ((fsubst'_body @ fsubst'_pre) # fsubst)) body1 body2 \<and>
+           list_all2 (alpha_equiv_statement' ((fsubst'_post @ fsubst'_pre) # fsubst)) post1 post2))))
     | _ \<Rightarrow> False)"
 
-| "alpha_equiv_statement' fsubst _
+| "alpha_equiv_statement' fsubst
   YulBreak stm2 =
   (case stm2 of
     YulBreak \<Rightarrow> True
     | _ \<Rightarrow> False)"
 
-| "alpha_equiv_statement' fsubst _
+| "alpha_equiv_statement' fsubst
   YulContinue stm2 =
   (case stm2 of
     YulContinue \<Rightarrow> True
     | _ \<Rightarrow> False)"
 
-| "alpha_equiv_statement' fsubst _
+| "alpha_equiv_statement' fsubst
   YulLeave stm2 =
   (case stm2 of
     YulLeave \<Rightarrow> True
     | _ \<Rightarrow> False)"
 
-| "alpha_equiv_statement' fsubst False
+(* should we not augment context here? *)
+| "alpha_equiv_statement' fsubst
   (YulBlock body1) stm2 =
   (case stm2 of
     (YulBlock body2) \<Rightarrow>
       (case alpha_equiv_check_decls body1 body2 of
         None \<Rightarrow> False
         | Some (fsubst') \<Rightarrow>
-          list_all2 (alpha_equiv_statement' (fsubst' # fsubst) False) body1 body2)
-    | _ \<Rightarrow> False)"
-
-| "alpha_equiv_statement' fsubst True
-  (YulBlock body1) stm2 =
-  (case stm2 of
-    (YulBlock body2) \<Rightarrow>
-      (case alpha_equiv_check_decls body1 body2 of
-        None \<Rightarrow> False
-        | Some (fsubst') \<Rightarrow>
-          list_all2 (alpha_equiv_statement' (fsubst) True) body1 body2)
+          list_all2 (alpha_equiv_statement' (fsubst' # fsubst)) body1 body2)
     | _ \<Rightarrow> False)"
 
 
-definition alpha_equiv_local ::
-  "subst \<Rightarrow> (YulIdentifier * 'v) \<Rightarrow> (YulIdentifier * 'v) \<Rightarrow> bool" where
-"alpha_equiv_local fsubst loc1 loc2 =
-  (case loc1 of (n1, v1) \<Rightarrow>
-  (case loc2 of (n2, v2) \<Rightarrow>
-  (v1 = v2 \<and> n1 = n2)))"
-
-(*
-definition alpha_equiv_locals' ::
-  "subst \<Rightarrow> (YulIdentifier * 'v) list \<Rightarrow> (YulIdentifier * 'v) list \<Rightarrow> bool" where
-"alpha_equiv_locals' fsubst locs1 locs2 =
-  list_all2 (alpha_equiv_local fsubst) locs1 locs2"
-*)
-
-definition alpha_equiv_locals' ::
-  "subst \<Rightarrow> (YulIdentifier * 'v) list \<Rightarrow> (YulIdentifier * 'v) list \<Rightarrow> bool" where
-"alpha_equiv_locals' fsubst locs1 locs2 =
-  (locs1 = locs2)"
-
-(*
-definition alpha_equiv_locals' ::
-  "subst \<Rightarrow> subst \<Rightarrow> 'v locals \<Rightarrow> 'v locals \<Rightarrow> bool" where
-"alpha_equiv_locals' vsubst fsubst [] [] = True"
-| "alpha_equiv_locals' vsubst fsubst ((n1, v1)#t1) ((n2, v2)#t2) =
-   (v1 = v2 \<and>
-    subst_lookup vsubst n1 = Some n2 \<and>
-    alpha_equiv_locals' vsubst fsubst t1 t2)"
-| "alpha_equiv_locals' _ _ _ _ = False"
-*)
-
-(* TODO: need equality of function parameters/returns here?
- * or just alpha equivalence?
- * i think alpha equivalence should suffice. but under what context?
- *)
 (* builtins need to be exactly equal.
- * TODO: perhaps revisit
  * TODO: can we get away with something weaker than alpha_equiv_statement' here?
  *  *)
 definition alpha_equiv_function_sig'_scheme ::
@@ -401,7 +440,7 @@ definition alpha_equiv_function_sig'_scheme ::
   (case (f_sig_body s1, f_sig_body s2) of
         (YulBuiltin b1, YulBuiltin b2) \<Rightarrow> s1 = s2
         | (YulFunction sts1, YulFunction sts2) \<Rightarrow>
-          alpha_equiv_statement' fsubst False
+          alpha_equiv_statement' fsubst
               (YulFunctionDefinitionStatement (YulFunctionDefinition n1 (f_sig_arguments s1) (f_sig_returns s1) sts1))
               (YulFunctionDefinitionStatement (YulFunctionDefinition n2 (f_sig_arguments s2) (f_sig_returns s2) sts2))
         | (_, _) \<Rightarrow> False)"
@@ -432,25 +471,18 @@ definition alpha_equiv_funs' ::
 "alpha_equiv_funs' fsubst funs1 funs2 =
   list_all2 (alpha_equiv_fun fsubst) funs1 funs2"
 
-(* TODO: make sure we are handling equivalence of function-contexts correctly.
- * this is a bit complicated to due to possibility of recursion/mutual recursion *)
 (* we are augmenting contexts twice when exiting statements.
  * this remains a problem for equivalence of funs (we augment once, should augment 0 times)
  *)
+
 fun alpha_equiv_stackEl' ::
   "subst \<Rightarrow> ('g, 'v, 't) StackEl \<Rightarrow> ('g, 'v, 't) StackEl \<Rightarrow> bool" where
 "alpha_equiv_stackEl' fsubst (EnterStatement s1) (EnterStatement s2) =
-  alpha_equiv_statement' fsubst False s1 s2"
-(* TODO: change this argument to True if we need different handling. *)
+  alpha_equiv_statement' fsubst s1 s2"
 | "alpha_equiv_stackEl' fsubst (ExitStatement s1 vs1 fs1) (ExitStatement s2 vs2 fs2) =
-    (let fsubst' =
-      (case s1 of
-        YulBlock _ \<Rightarrow> List.tl (fsubst)
-        | _ \<Rightarrow> fsubst)
-     in
-      (alpha_equiv_statement' fsubst' False s1 s2 \<and>
-       alpha_equiv_locals' fsubst' vs1 vs2 \<and>
-       alpha_equiv_funs' fsubst' fs1 fs2))"
+      (alpha_equiv_statement' fsubst s1 s2 \<and>
+       alpha_equiv_locals' fsubst vs1 vs2 \<and>
+       alpha_equiv_funs' fsubst fs1 fs2)"
 | "alpha_equiv_stackEl' fsubst (Expression e1) (Expression e2) =
   alpha_equiv_expr' fsubst e1 e2"
 | "alpha_equiv_stackEl' fsubst (EnterFunctionCall n1 f1) (EnterFunctionCall n2 f2) = 
@@ -462,69 +494,127 @@ fun alpha_equiv_stackEl' ::
      alpha_equiv_funs' fsubst fs1 fs2)"
 | "alpha_equiv_stackEl' fsubst _ _ = False"
 
-(* whenever we extend the variable context, we also need to update subst.  *)
-(* also need to update subst on function entry. *)
+(* use subst_update in order to ensure that we maintain the correct substitution *)
+(* should we do subst_update on head also? or just tail? neither? *)
 
-(* gather yul functions / get_fun_decls *)
+fun alpha_equiv_stackEls' ::
+  "subst \<Rightarrow> ('g, 'v, 't) StackEl list \<Rightarrow> ('g, 'v, 't) StackEl list \<Rightarrow> bool" where
+"alpha_equiv_stackEls' fsubst [] [] = True"
+| "alpha_equiv_stackEls' fsubst (h1#t1) (h2#t2) =
+   (case subst_updatex fsubst h1 h2 of
+    None \<Rightarrow> False
+    | Some fsubst' \<Rightarrow>
+    (alpha_equiv_stackEl' fsubst' h1 h2 \<and>
+      alpha_equiv_stackEls' fsubst' t1 t2))"
+| "alpha_equiv_stackEls' fsubst _ _ = False"
 
-fun subst_update_enter_statement ::
-  "subst \<Rightarrow> 
-   ('v, 't) YulStatement \<Rightarrow>
-   ('v, 't) YulStatement \<Rightarrow>
-   (subst)" where
-"subst_update_enter_statement fsubst (YulBlock ls1) (YulBlock ls2) =
-  ((zip (get_fun_decls ls1) (get_fun_decls ls2))# fsubst)"
-| "subst_update_enter_statement fsubst _ _ = (fsubst)"
+(* used for splitting apart alpha_equiv_stackEls' *)
+fun alpha_equiv_stackEls'_newsubst ::
+  "subst \<Rightarrow> ('g, 'v, 't) StackEl list \<Rightarrow> ('g, 'v, 't) StackEl list \<Rightarrow> subst option" where
+"alpha_equiv_stackEls'_newsubst fsubst [] [] = Some fsubst"
+| "alpha_equiv_stackEls'_newsubst fsubst (h1#t1) (h2#t2) =
+   (case subst_updatex fsubst h1 h2 of
+    None \<Rightarrow> None
+    | Some fsubst' \<Rightarrow>
+      alpha_equiv_stackEls'_newsubst fsubst' t1 t2)"
+| "alpha_equiv_stackEls'_newsubst fsubst _ _ = None"
+
+(* TODO *)
+lemma alpha_equiv_stackEls'_split :
+  assumes "alpha_equiv_stackEls' fsubst pre1 pre2"
+  assumes "alpha_equiv_stackEls'_newsubst fsubst pre1 pre2 = Some fsubst'"
+  assumes "alpha_equiv_stackEls' fsubst' post1 post2"
+  shows "alpha_equiv_stackEls' fsubst (pre1 @ post1) (pre2 @ post2)"
+using assms
+proof(induction pre1 arbitrary: fsubst pre2 fsubst' post1 post2)
+  case Nil1 : Nil
+
+  have Nil2 : "pre2 = []"
+    using Nil1
+    by(cases pre2; auto)
+
+  show ?case
+    using Nil1 Nil2
+    by(auto)
+next
+  case Cons1 : (Cons preh1 pret1)
+
+  obtain preh2 pret2 where Cons2 : "pre2 = preh2 # pret2"
+    using Cons1.prems
+    by(cases pre2; auto)
+
+  show ?case
+  proof(cases preh1)
+    case ES1 : (EnterStatement s1)
+
+    obtain s2 where ES2 : "preh2 = (EnterStatement s2)"
+      using ES1 Cons1.prems Cons2
+      by (cases preh2; auto)
+
+    then show ?thesis
+      using Cons1 Cons2 ES1 ES2
+      by(cases s1; auto)
+  next
+    case XS1 : (ExitStatement s1 locals1 funcs1)
+
+    then obtain s2 locals2 funcs2 where XS2 :
+      "preh2 = ExitStatement s2 locals2 funcs2"
+      using Cons1.prems Cons2
+      by(cases preh2; auto)
+
+    obtain fsubst' where Fsubst' :
+      "subst_updatex_exit_statement fsubst s1 s2 = Some fsubst'"
+      using Cons1 Cons2 XS1 XS2
+      by(cases "subst_updatex_exit_statement fsubst s1 s2"; auto)
+
+    show ?thesis using Cons1 Cons2 XS1 XS2 Fsubst'
+      by(auto)
+  next
+    case EF1 : (EnterFunctionCall name1 sig1)
+
+    then obtain name2 sig2 where EF2:
+      "preh2 = EnterFunctionCall name2 sig2"
+      using EF1 Cons1.prems Cons2
+      by(cases preh2; auto)
+
+    show ?thesis
+      using Cons1 Cons2 EF1 EF2
+      by(auto)
+  next
+    case XF1 : (ExitFunctionCall name1 vals1 locals1 funcs1 f1)
+    then obtain name2 vals2 locals2 funcs2 f2 where XF2 :
+      "preh2 = ExitFunctionCall name2 vals2 locals2 funcs2 f2"
+      using XF1 Cons1.prems Cons2
+      by(cases preh2; auto)
+
+    obtain fsubst' where Fsubst' :
+      "subst_updatex_exit_fun_call fsubst = Some fsubst'"
+      using Cons1 Cons2 XF1 XF2
+      by(cases "subst_updatex_exit_fun_call fsubst"; auto)
+
+    show ?thesis using Cons1 Cons2 XF1 XF2 Fsubst'
+      by(auto)
+  next
+    case Exp1 : (Expression e1)
+
+    obtain e2 where Exp2 : "preh2 = (Expression e2)"
+      using Exp1 Cons1.prems Cons2
+      by (cases preh2; auto)
+
+    show ?thesis
+      using Cons1 Cons2 Exp1 Exp2
+      by(cases e1; auto)
+  qed
+qed
+
+
 
 (*
-fun YulStatement_same_constr ::
-  "('v, 't) YulStatement \<Rightarrow> ('v, 't) YulStatement \<Rightarrow> bool" where
-
-| "YulStatement_same_constr _ _ = False"
+abbreviation (input) alpha_equiv_stackEls' ::
+  "subst \<Rightarrow> ('g, 'v, 't) StackEl list \<Rightarrow> ('g, 'v, 't) StackEl list \<Rightarrow> bool" where
+"alpha_equiv_stackEls' fsubst l1 l2 \<equiv>
+  list_all2 (alpha_equiv_stackEl' fsubst) l1 l2"
 *)
-fun subst_update_exit_statement ::
-  "subst \<Rightarrow> 
-   ('v, 't) YulStatement \<Rightarrow>
-   ('v, 't) YulStatement \<Rightarrow>
-   (subst) option" where
-"subst_update_exit_statement fsubst
-  (YulVariableDeclarationStatement (YulVariableDeclaration ns1 eo1))
-  (YulVariableDeclarationStatement (YulVariableDeclaration ns2 eo2)) = Some fsubst"
-| "subst_update_exit_statement fsubst
-  (YulBlock ls1)
-  (YulBlock ls2) = 
-  (case (fsubst) of
-    (fsh # fsubst') \<Rightarrow> Some (fsubst')
-   | _ \<Rightarrow> None)"
-(* bogus cases mixed with noop cases here. *)
-| "subst_update_exit_statement fsubst _ _ = Some (fsubst)" 
-
-fun subst_update_enter_fun_call ::
-    "subst \<Rightarrow> ('g, 'v, 't, 'z) function_sig'_scheme \<Rightarrow> ('g, 'v, 't, 'z) function_sig'_scheme \<Rightarrow> (subst)"
-    where
-  "subst_update_enter_fun_call fsubst
-    sig1 sig2 = fsubst
-    "
-
-(* TODO: is this correct or should we leave fsubst unchanged? *)
-fun subst_update_exit_fun_call ::
-  "subst \<Rightarrow>  (subst) option"
-  where
-"subst_update_exit_fun_call (fsh # fsubst') = Some (fsubst')"
-| "subst_update_exit_fun_call fsubst = None"
-
-(* TODO: return an option? *)
-fun subst_update ::
-  "subst \<Rightarrow> ('g, 'v, 't) StackEl \<Rightarrow> ('g, 'v, 't) StackEl \<Rightarrow> (subst) option" where
-"subst_update fsubst (EnterStatement s1) (EnterStatement s2) =
-  Some (subst_update_enter_statement fsubst s1 s2)"
-| "subst_update fsubst (ExitStatement s1 _ _) (ExitStatement s2 _ _) =
-  subst_update_exit_statement fsubst s1 s2"
-| "subst_update fsubst (EnterFunctionCall f1 s1) (EnterFunctionCall f2 s2) =
-  Some (subst_update_enter_fun_call fsubst s1 s2)"
-| "subst_update fsubst (ExitFunctionCall _ _ _ _ _) (ExitFunctionCall _ _ _ _ _) = 
-  subst_update_exit_fun_call fsubst"
-| "subst_update fsubst _ _ = Some (fsubst)"
 
 definition alpha_equiv_results' ::
   "subst \<Rightarrow>
@@ -536,7 +626,7 @@ definition alpha_equiv_results' ::
    vals r1 = vals r2 \<and>
    locals r1 = locals r2 \<and>
    alpha_equiv_funs' fsubst (funs r1) (funs r2) \<and>
-   (list_all2 (alpha_equiv_stackEl' fsubst)
+   (alpha_equiv_stackEls' fsubst
               (cont r1)
               (cont r2)))"
 
@@ -643,1271 +733,9 @@ next
 
   show ?case using Cons1.prems Cons1.IH[OF Tl] Cons2
     by(auto)
-qed
-(*
-lemma alpha_equiv_funs_trunc :
-  assumes H: "alpha_equiv_funs' fsubst funs1 funs2"
-  shows "alpha_equiv_funs' fsubst
-     (map (\<lambda>(n, fs). (n, function_sig'.truncate fs)) funs1)
-     (map (\<lambda>(n, fs). (n, function_sig'.truncate fs)) funs2)"
-  using alpha_equiv_fun_trunc H
-  unfolding alpha_equiv_funs'_def
-  using list_all2_map[of "alpha_equiv_fun fsubst" _ _
-      "alpha_equiv_fun fsubst"
-      "(\<lambda>(n, fs). (n, function_sig'.truncate fs))"
-      "(\<lambda>(n, fs). (n, function_sig'.truncate fs))"]
-  by(blast)
-*)
-(*
-lemma alpha_equiv_check_decls_cases :
-  assumes H: "alpha_equiv_check_decls l1 l2 = Some x"
-  shows
-    "(l1 = [] \<and> l2 = [] \<and> x = ([], [])) \<or>
-     (\<exists> l1h l1t l2h l2t fs vs . x = (vs, fs) \<and>
-      l1 = l1h # l1t \<and> l2 = l2h # l2t \<and> yul_statement_same_constructor l1h l2h \<and> 
-      (\<exists> decls1 v1 decls2 v2 vs' .
-        l1h = (YulVariableDeclarationStatement (YulVariableDeclaration decls1 v1)) \<and>
-        l2h = (YulVariableDeclarationStatement (YulVariableDeclaration decls2 v2)) \<and>
-        alpha_equiv_check_decls l1t l2t = Some (vs', fs) \<and>
-        vs = ((zip (map (\<lambda> x . case x of (YulTypedName n _) \<Rightarrow> n) decls1)
-                   (map (\<lambda> x . case x of (YulTypedName n _) \<Rightarrow> n) decls2)) @ vs')) \<or>
-      (\<exists> name1 args1 rets1 body1 name2 args2 rets2 body2 fs' .
-        l1h = (YulFunctionDefinitionStatement (YulFunctionDefinition name1 args1 rets1 body1)) \<and>
-        l2h = (YulFunctionDefinitionStatement (YulFunctionDefinition name2 args2 rets2 body2)) \<and>
-        alpha_equiv_check_decls l1t l2t = Some (vs, fs') \<and>
-        fs = (name1, name2)#fs') \<or>
-      ((case l1h of
-        YulVariableDeclarationStatement _ \<Rightarrow> False
-        | YulFunctionDefinitionStatement _ \<Rightarrow> False
-        | _ \<Rightarrow> True) \<and>
-       (case l2h of
-        YulVariableDeclarationStatement _ \<Rightarrow> False
-        | YulFunctionDefinitionStatement _ \<Rightarrow> False
-        | _ \<Rightarrow> True) \<and> alpha_equiv_check_decls l1t l2t = Some x))"
-
-proof(cases l1)
-  case Nil
-  then show ?thesis using H
-    by(cases l2; auto)
 next
-  case C1: (Cons l1h l1t)
-
-  then obtain l2h l2t where C2 :
-    "l2 = l2h # l2t"
-    using H
-    by(cases l2; auto)
-
-  obtain x1 x2 where X: "x = (x1, x2)"
-    by(cases x; auto)
-
-  show ?thesis
-  proof(cases l1h)
-    case (YulFunctionCallStatement x1)
-
-    then have "(\<exists>l1h l1t l2h l2t fs vs.
-        x = (vs, fs) \<and>
-        l1 = l1h # l1t \<and>
-        l2 = l2h # l2t \<and>
-        yul_statement_same_constructor l1h l2h \<and>
-        (case l1h of YulVariableDeclarationStatement x \<Rightarrow> False
-         | YulFunctionDefinitionStatement x \<Rightarrow> False
-         | _ \<Rightarrow> True) \<and>
-        (case l2h of YulVariableDeclarationStatement x \<Rightarrow> False
-         | YulFunctionDefinitionStatement x \<Rightarrow> False
-         | _ \<Rightarrow> True) \<and>
-        alpha_equiv_check_decls l1t l2t = Some x)" using H C1 C2 X
-      by(cases l2h; auto)
-
-    then show ?thesis by blast
-  next
-    case (YulAssignmentStatement x2)
-    then have "(\<exists>l1h l1t l2h l2t fs vs.
-        x = (vs, fs) \<and>
-        l1 = l1h # l1t \<and>
-        l2 = l2h # l2t \<and>
-        yul_statement_same_constructor l1h l2h \<and>
-        (case l1h of YulVariableDeclarationStatement x \<Rightarrow> False
-         | YulFunctionDefinitionStatement x \<Rightarrow> False
-         | _ \<Rightarrow> True) \<and>
-        (case l2h of YulVariableDeclarationStatement x \<Rightarrow> False
-         | YulFunctionDefinitionStatement x \<Rightarrow> False
-         | _ \<Rightarrow> True) \<and>
-        alpha_equiv_check_decls l1t l2t = Some x)" using H C1 C2 X
-      by(cases l2h; auto)
-
-    then show ?thesis by blast
-  next
-    case L1h : (YulVariableDeclarationStatement vds)
-
-    then obtain vds' where L2h : "l2h = YulVariableDeclarationStatement vds'"
-      using H C1 C2 X
-      by(cases l2h; auto)
-
-    then have Conc' : "(\<exists> l1h l1t l2h l2t fs vs . x = (vs, fs) \<and>
-      l1 = l1h # l1t \<and> l2 = l2h # l2t \<and> yul_statement_same_constructor l1h l2h \<and> 
-      (\<exists> decls1 v1 decls2 v2 vs' .
-        l1h = (YulVariableDeclarationStatement (YulVariableDeclaration decls1 v1)) \<and>
-        l2h = (YulVariableDeclarationStatement (YulVariableDeclaration decls2 v2)) \<and>
-        alpha_equiv_check_decls l1t l2t = Some (vs', fs) \<and>
-        vs = ((zip (map (\<lambda> x . case x of (YulTypedName n _) \<Rightarrow> n) decls1)
-                   (map (\<lambda> x . case x of (YulTypedName n _) \<Rightarrow> n) decls2)) @ vs')))"
-      using H C1 C2 X L1h
-      by(cases vds; cases vds'; auto split: option.splits if_splits)
-
-    then show ?thesis by metis
-      
-  next
-    case L1h : (YulFunctionDefinitionStatement fds)
-
-    then obtain fds' where L2h : "l2h = YulFunctionDefinitionStatement fds'"
-      using H C1 C2 X
-      by(cases l2h; auto)
-
-    then have Conc' : "(\<exists> l1h l1t l2h l2t fs vs . x = (vs, fs) \<and>
-      l1 = l1h # l1t \<and> l2 = l2h # l2t \<and> yul_statement_same_constructor l1h l2h \<and> 
-      (\<exists> name1 args1 rets1 body1 name2 args2 rets2 body2 fs' .
-        l1h = (YulFunctionDefinitionStatement (YulFunctionDefinition name1 args1 rets1 body1)) \<and>
-        l2h = (YulFunctionDefinitionStatement (YulFunctionDefinition name2 args2 rets2 body2)) \<and>
-        alpha_equiv_check_decls l1t l2t = Some (vs, fs') \<and>
-        fs = (name1, name2)#fs'))"
-      using H C1 C2 X L1h
-      by(cases fds; cases fds'; auto split: option.splits if_splits)
-
-    then show ?thesis by metis
-  next
-    case (YulIf x51 x52)
-    then have "(\<exists>l1h l1t l2h l2t fs vs.
-        x = (vs, fs) \<and>
-        l1 = l1h # l1t \<and>
-        l2 = l2h # l2t \<and>
-        yul_statement_same_constructor l1h l2h \<and>
-        (case l1h of YulVariableDeclarationStatement x \<Rightarrow> False
-         | YulFunctionDefinitionStatement x \<Rightarrow> False
-         | _ \<Rightarrow> True) \<and>
-        (case l2h of YulVariableDeclarationStatement x \<Rightarrow> False
-         | YulFunctionDefinitionStatement x \<Rightarrow> False
-         | _ \<Rightarrow> True) \<and>
-        alpha_equiv_check_decls l1t l2t = Some x)" using H C1 C2 X
-      by(cases l2h; auto)
-
-    then show ?thesis by blast
-  next
-    case (YulSwitch x61 x62)
-    then have "(\<exists>l1h l1t l2h l2t fs vs.
-        x = (vs, fs) \<and>
-        l1 = l1h # l1t \<and>
-        l2 = l2h # l2t \<and>
-        yul_statement_same_constructor l1h l2h \<and>
-        (case l1h of YulVariableDeclarationStatement x \<Rightarrow> False
-         | YulFunctionDefinitionStatement x \<Rightarrow> False
-         | _ \<Rightarrow> True) \<and>
-        (case l2h of YulVariableDeclarationStatement x \<Rightarrow> False
-         | YulFunctionDefinitionStatement x \<Rightarrow> False
-         | _ \<Rightarrow> True) \<and>
-        alpha_equiv_check_decls l1t l2t = Some x)" using H C1 C2 X
-      by(cases l2h; auto)
-
-    then show ?thesis by blast
-  next
-    case (YulForLoop x71 x72 x73 x74)
-    then have "(\<exists>l1h l1t l2h l2t fs vs.
-        x = (vs, fs) \<and>
-        l1 = l1h # l1t \<and>
-        l2 = l2h # l2t \<and>
-        yul_statement_same_constructor l1h l2h \<and>
-        (case l1h of YulVariableDeclarationStatement x \<Rightarrow> False
-         | YulFunctionDefinitionStatement x \<Rightarrow> False
-         | _ \<Rightarrow> True) \<and>
-        (case l2h of YulVariableDeclarationStatement x \<Rightarrow> False
-         | YulFunctionDefinitionStatement x \<Rightarrow> False
-         | _ \<Rightarrow> True) \<and>
-        alpha_equiv_check_decls l1t l2t = Some x)" using H C1 C2 X
-      by(cases l2h; auto)
-
-    then show ?thesis by blast
-  next
-    case YulBreak
-    then have "(\<exists>l1h l1t l2h l2t fs vs.
-        x = (vs, fs) \<and>
-        l1 = l1h # l1t \<and>
-        l2 = l2h # l2t \<and>
-        yul_statement_same_constructor l1h l2h \<and>
-        (case l1h of YulVariableDeclarationStatement x \<Rightarrow> False
-         | YulFunctionDefinitionStatement x \<Rightarrow> False
-         | _ \<Rightarrow> True) \<and>
-        (case l2h of YulVariableDeclarationStatement x \<Rightarrow> False
-         | YulFunctionDefinitionStatement x \<Rightarrow> False
-         | _ \<Rightarrow> True) \<and>
-        alpha_equiv_check_decls l1t l2t = Some x)" using H C1 C2 X
-      by(cases l2h; auto)
-
-    then show ?thesis by blast
-  next
-  case YulContinue
-    then have "(\<exists>l1h l1t l2h l2t fs vs.
-        x = (vs, fs) \<and>
-        l1 = l1h # l1t \<and>
-        l2 = l2h # l2t \<and>
-        yul_statement_same_constructor l1h l2h \<and>
-        (case l1h of YulVariableDeclarationStatement x \<Rightarrow> False
-         | YulFunctionDefinitionStatement x \<Rightarrow> False
-         | _ \<Rightarrow> True) \<and>
-        (case l2h of YulVariableDeclarationStatement x \<Rightarrow> False
-         | YulFunctionDefinitionStatement x \<Rightarrow> False
-         | _ \<Rightarrow> True) \<and>
-        alpha_equiv_check_decls l1t l2t = Some x)" using H C1 C2 X
-      by(cases l2h; auto)
-
-    then show ?thesis by blast
-  next
-    case YulLeave
-    then have "(\<exists>l1h l1t l2h l2t fs vs.
-        x = (vs, fs) \<and>
-        l1 = l1h # l1t \<and>
-        l2 = l2h # l2t \<and>
-        yul_statement_same_constructor l1h l2h \<and>
-        (case l1h of YulVariableDeclarationStatement x \<Rightarrow> False
-         | YulFunctionDefinitionStatement x \<Rightarrow> False
-         | _ \<Rightarrow> True) \<and>
-        (case l2h of YulVariableDeclarationStatement x \<Rightarrow> False
-         | YulFunctionDefinitionStatement x \<Rightarrow> False
-         | _ \<Rightarrow> True) \<and>
-        alpha_equiv_check_decls l1t l2t = Some x)" using H C1 C2 X
-      by(cases l2h; auto)
-
-    then show ?thesis by blast
-  next
-    case (YulBlock x11)
-    then have "(\<exists>l1h l1t l2h l2t fs vs.
-        x = (vs, fs) \<and>
-        l1 = l1h # l1t \<and>
-        l2 = l2h # l2t \<and>
-        yul_statement_same_constructor l1h l2h \<and>
-        (case l1h of YulVariableDeclarationStatement x \<Rightarrow> False
-         | YulFunctionDefinitionStatement x \<Rightarrow> False
-         | _ \<Rightarrow> True) \<and>
-        (case l2h of YulVariableDeclarationStatement x \<Rightarrow> False
-         | YulFunctionDefinitionStatement x \<Rightarrow> False
-         | _ \<Rightarrow> True) \<and>
-        alpha_equiv_check_decls l1t l2t = Some x)" using H C1 C2 X
-      by(cases l2h; auto)
-
-    then show ?thesis by blast
-  qed
 qed
 
-lemma alpha_equiv_check_decls_cases_alt :
-  assumes H: "alpha_equiv_check_decls l1 l2 = Some x"
-  shows
-    "(l1 = [] \<and> l2 = [] \<and> x = ([], [])) \<or>
-     (\<exists> l1h l1t l2h l2t fs vs decls1 v1 decls2 v2 vs' . x = (vs, fs) \<and>
-      l1 = l1h # l1t \<and> l2 = l2h # l2t \<and> yul_statement_same_constructor l1h l2h \<and> 
-        l1h = (YulVariableDeclarationStatement (YulVariableDeclaration decls1 v1)) \<and>
-        l2h = (YulVariableDeclarationStatement (YulVariableDeclaration decls2 v2)) \<and>
-        alpha_equiv_check_decls l1t l2t = Some (vs', fs) \<and>
-        vs = ((zip (map (\<lambda> x . case x of (YulTypedName n _) \<Rightarrow> n) decls1)
-                   (map (\<lambda> x . case x of (YulTypedName n _) \<Rightarrow> n) decls2)) @ vs')) \<or>
-      (\<exists> l1h l1t l2h l2t fs vs name1 args1 rets1 body1 name2 args2 rets2 body2 fs' . x = (vs, fs) \<and>
-        l1 = l1h # l1t \<and> l2 = l2h # l2t \<and> yul_statement_same_constructor l1h l2h \<and> 
-        l1h = (YulFunctionDefinitionStatement (YulFunctionDefinition name1 args1 rets1 body1)) \<and>
-        l2h = (YulFunctionDefinitionStatement (YulFunctionDefinition name2 args2 rets2 body2)) \<and>
-        alpha_equiv_check_decls l1t l2t = Some (vs, fs') \<and>
-        fs = (name1, name2)#fs') \<or>
-      (\<exists> l1h l1t l2h l2t fs vs . x = (vs, fs) \<and>
-      l1 = l1h # l1t \<and> l2 = l2h # l2t \<and> yul_statement_same_constructor l1h l2h \<and>
-      (case l1h of
-        YulVariableDeclarationStatement _ \<Rightarrow> False
-        | YulFunctionDefinitionStatement _ \<Rightarrow> False
-        | _ \<Rightarrow> True) \<and>
-       (case l2h of
-        YulVariableDeclarationStatement _ \<Rightarrow> False
-        | YulFunctionDefinitionStatement _ \<Rightarrow> False
-        | _ \<Rightarrow> True) \<and> alpha_equiv_check_decls l1t l2t = Some x)"
-proof(cases l1)
-  case Nil
-  then show ?thesis using H
-    by(cases l2; auto)
-next
-  case C1: (Cons l1h l1t)
-
-  then obtain l2h l2t where C2 :
-    "l2 = l2h # l2t"
-    using H
-    by(cases l2; auto)
-
-  obtain x1 x2 where X: "x = (x1, x2)"
-    by(cases x; auto)
-
-  show ?thesis
-  proof(cases l1h)
-    case (YulFunctionCallStatement x1)
-
-    then have "(\<exists>l1h l1t l2h l2t fs vs.
-        x = (vs, fs) \<and>
-        l1 = l1h # l1t \<and>
-        l2 = l2h # l2t \<and>
-        yul_statement_same_constructor l1h l2h \<and>
-        (case l1h of YulVariableDeclarationStatement x \<Rightarrow> False
-         | YulFunctionDefinitionStatement x \<Rightarrow> False
-         | _ \<Rightarrow> True) \<and>
-        (case l2h of YulVariableDeclarationStatement x \<Rightarrow> False
-         | YulFunctionDefinitionStatement x \<Rightarrow> False
-         | _ \<Rightarrow> True) \<and>
-        alpha_equiv_check_decls l1t l2t = Some x)" using H C1 C2 X
-      by(cases l2h; auto)
-
-    then show ?thesis by blast
-  next
-    case (YulAssignmentStatement x2)
-    then have "(\<exists>l1h l1t l2h l2t fs vs.
-        x = (vs, fs) \<and>
-        l1 = l1h # l1t \<and>
-        l2 = l2h # l2t \<and>
-        yul_statement_same_constructor l1h l2h \<and>
-        (case l1h of YulVariableDeclarationStatement x \<Rightarrow> False
-         | YulFunctionDefinitionStatement x \<Rightarrow> False
-         | _ \<Rightarrow> True) \<and>
-        (case l2h of YulVariableDeclarationStatement x \<Rightarrow> False
-         | YulFunctionDefinitionStatement x \<Rightarrow> False
-         | _ \<Rightarrow> True) \<and>
-        alpha_equiv_check_decls l1t l2t = Some x)" using H C1 C2 X
-      by(cases l2h; auto)
-
-    then show ?thesis by blast
-  next
-    case L1h : (YulVariableDeclarationStatement vds)
-
-    then obtain vds' where L2h : "l2h = YulVariableDeclarationStatement vds'"
-      using H C1 C2 X
-      by(cases l2h; auto)
-
-    then have Conc' : "(\<exists> l1h l1t l2h l2t fs vs . x = (vs, fs) \<and>
-      l1 = l1h # l1t \<and> l2 = l2h # l2t \<and> yul_statement_same_constructor l1h l2h \<and> 
-      (\<exists> decls1 v1 decls2 v2 vs' .
-        l1h = (YulVariableDeclarationStatement (YulVariableDeclaration decls1 v1)) \<and>
-        l2h = (YulVariableDeclarationStatement (YulVariableDeclaration decls2 v2)) \<and>
-        alpha_equiv_check_decls l1t l2t = Some (vs', fs) \<and>
-        vs = ((zip (map (\<lambda> x . case x of (YulTypedName n _) \<Rightarrow> n) decls1)
-                   (map (\<lambda> x . case x of (YulTypedName n _) \<Rightarrow> n) decls2)) @ vs')))"
-      using H C1 C2 X L1h
-      by(cases vds; cases vds'; auto split: option.splits if_splits)
-
-    then show ?thesis by metis
-      
-  next
-    case L1h : (YulFunctionDefinitionStatement fds)
-
-    then obtain fds' where L2h : "l2h = YulFunctionDefinitionStatement fds'"
-      using H C1 C2 X
-      by(cases l2h; auto)
-
-    then have Conc' : "(\<exists> l1h l1t l2h l2t fs vs . x = (vs, fs) \<and>
-      l1 = l1h # l1t \<and> l2 = l2h # l2t \<and> yul_statement_same_constructor l1h l2h \<and> 
-      (\<exists> name1 args1 rets1 body1 name2 args2 rets2 body2 fs' .
-        l1h = (YulFunctionDefinitionStatement (YulFunctionDefinition name1 args1 rets1 body1)) \<and>
-        l2h = (YulFunctionDefinitionStatement (YulFunctionDefinition name2 args2 rets2 body2)) \<and>
-        alpha_equiv_check_decls l1t l2t = Some (vs, fs') \<and>
-        fs = (name1, name2)#fs'))"
-      using H C1 C2 X L1h
-      by(cases fds; cases fds'; auto split: option.splits if_splits)
-
-    then show ?thesis by metis
-  next
-    case (YulIf x51 x52)
-    then have "(\<exists>l1h l1t l2h l2t fs vs.
-        x = (vs, fs) \<and>
-        l1 = l1h # l1t \<and>
-        l2 = l2h # l2t \<and>
-        yul_statement_same_constructor l1h l2h \<and>
-        (case l1h of YulVariableDeclarationStatement x \<Rightarrow> False
-         | YulFunctionDefinitionStatement x \<Rightarrow> False
-         | _ \<Rightarrow> True) \<and>
-        (case l2h of YulVariableDeclarationStatement x \<Rightarrow> False
-         | YulFunctionDefinitionStatement x \<Rightarrow> False
-         | _ \<Rightarrow> True) \<and>
-        alpha_equiv_check_decls l1t l2t = Some x)" using H C1 C2 X
-      by(cases l2h; auto)
-
-    then show ?thesis by blast
-  next
-    case (YulSwitch x61 x62)
-    then have "(\<exists>l1h l1t l2h l2t fs vs.
-        x = (vs, fs) \<and>
-        l1 = l1h # l1t \<and>
-        l2 = l2h # l2t \<and>
-        yul_statement_same_constructor l1h l2h \<and>
-        (case l1h of YulVariableDeclarationStatement x \<Rightarrow> False
-         | YulFunctionDefinitionStatement x \<Rightarrow> False
-         | _ \<Rightarrow> True) \<and>
-        (case l2h of YulVariableDeclarationStatement x \<Rightarrow> False
-         | YulFunctionDefinitionStatement x \<Rightarrow> False
-         | _ \<Rightarrow> True) \<and>
-        alpha_equiv_check_decls l1t l2t = Some x)" using H C1 C2 X
-      by(cases l2h; auto)
-
-    then show ?thesis by blast
-  next
-    case (YulForLoop x71 x72 x73 x74)
-    then have "(\<exists>l1h l1t l2h l2t fs vs.
-        x = (vs, fs) \<and>
-        l1 = l1h # l1t \<and>
-        l2 = l2h # l2t \<and>
-        yul_statement_same_constructor l1h l2h \<and>
-        (case l1h of YulVariableDeclarationStatement x \<Rightarrow> False
-         | YulFunctionDefinitionStatement x \<Rightarrow> False
-         | _ \<Rightarrow> True) \<and>
-        (case l2h of YulVariableDeclarationStatement x \<Rightarrow> False
-         | YulFunctionDefinitionStatement x \<Rightarrow> False
-         | _ \<Rightarrow> True) \<and>
-        alpha_equiv_check_decls l1t l2t = Some x)" using H C1 C2 X
-      by(cases l2h; auto)
-
-    then show ?thesis by blast
-  next
-    case YulBreak
-    then have "(\<exists>l1h l1t l2h l2t fs vs.
-        x = (vs, fs) \<and>
-        l1 = l1h # l1t \<and>
-        l2 = l2h # l2t \<and>
-        yul_statement_same_constructor l1h l2h \<and>
-        (case l1h of YulVariableDeclarationStatement x \<Rightarrow> False
-         | YulFunctionDefinitionStatement x \<Rightarrow> False
-         | _ \<Rightarrow> True) \<and>
-        (case l2h of YulVariableDeclarationStatement x \<Rightarrow> False
-         | YulFunctionDefinitionStatement x \<Rightarrow> False
-         | _ \<Rightarrow> True) \<and>
-        alpha_equiv_check_decls l1t l2t = Some x)" using H C1 C2 X
-      by(cases l2h; auto)
-
-    then show ?thesis by blast
-  next
-  case YulContinue
-    then have "(\<exists>l1h l1t l2h l2t fs vs.
-        x = (vs, fs) \<and>
-        l1 = l1h # l1t \<and>
-        l2 = l2h # l2t \<and>
-        yul_statement_same_constructor l1h l2h \<and>
-        (case l1h of YulVariableDeclarationStatement x \<Rightarrow> False
-         | YulFunctionDefinitionStatement x \<Rightarrow> False
-         | _ \<Rightarrow> True) \<and>
-        (case l2h of YulVariableDeclarationStatement x \<Rightarrow> False
-         | YulFunctionDefinitionStatement x \<Rightarrow> False
-         | _ \<Rightarrow> True) \<and>
-        alpha_equiv_check_decls l1t l2t = Some x)" using H C1 C2 X
-      by(cases l2h; auto)
-
-    then show ?thesis by blast
-  next
-    case YulLeave
-    then have "(\<exists>l1h l1t l2h l2t fs vs.
-        x = (vs, fs) \<and>
-        l1 = l1h # l1t \<and>
-        l2 = l2h # l2t \<and>
-        yul_statement_same_constructor l1h l2h \<and>
-        (case l1h of YulVariableDeclarationStatement x \<Rightarrow> False
-         | YulFunctionDefinitionStatement x \<Rightarrow> False
-         | _ \<Rightarrow> True) \<and>
-        (case l2h of YulVariableDeclarationStatement x \<Rightarrow> False
-         | YulFunctionDefinitionStatement x \<Rightarrow> False
-         | _ \<Rightarrow> True) \<and>
-        alpha_equiv_check_decls l1t l2t = Some x)" using H C1 C2 X
-      by(cases l2h; auto)
-
-    then show ?thesis by blast
-  next
-    case (YulBlock x11)
-    then have "(\<exists>l1h l1t l2h l2t fs vs.
-        x = (vs, fs) \<and>
-        l1 = l1h # l1t \<and>
-        l2 = l2h # l2t \<and>
-        yul_statement_same_constructor l1h l2h \<and>
-        (case l1h of YulVariableDeclarationStatement x \<Rightarrow> False
-         | YulFunctionDefinitionStatement x \<Rightarrow> False
-         | _ \<Rightarrow> True) \<and>
-        (case l2h of YulVariableDeclarationStatement x \<Rightarrow> False
-         | YulFunctionDefinitionStatement x \<Rightarrow> False
-         | _ \<Rightarrow> True) \<and>
-        alpha_equiv_check_decls l1t l2t = Some x)" using H C1 C2 X
-      by(cases l2h; auto)
-
-    then show ?thesis by blast
-  qed
-qed
-
-lemma alpha_equiv_check_decls_result :
-  assumes Decls : "alpha_equiv_check_decls sts1 sts2 = Some (locs', funcs')"
-  shows "\<exists> vs1 fs1 vs2 fs2 . 
-    length sts1 = length sts2 \<and>
-    get_var_decls sts1 = (map fst locs') \<and>
-    get_var_decls sts2 = (map snd locs') \<and>
-    get_fun_decls sts1 = (map fst funcs') \<and>
-    get_fun_decls sts2 = (map snd funcs')"
-  using assms
-proof(induction sts1 arbitrary: sts2 locs' funcs')
-  case Nil
-  then show ?case 
-    by(cases sts2; auto)
-next
-  case Cons1 : (Cons sts1h sts1t)
-
-  then obtain sts2h sts2t where Cons2 :
-    "sts2 = sts2h # sts2t"
-    using Cons1.prems
-    by(cases sts2; auto)
-
-  consider 
-    (1) "(sts1h#sts1t = [] \<and> sts2 = [] \<and> (locs', funcs') = ([], []))" |
-    (2) l1h l1t l2h l2t fs vs decls1 v1 decls2 v2 vs' where 
-      "(locs', funcs') = (vs, fs)"
-      "sts1h#sts1t  = l1h # l1t"
-      "sts2 = l2h # l2t"
-      "yul_statement_same_constructor l1h l2h"
-      "l1h = (YulVariableDeclarationStatement (YulVariableDeclaration decls1 v1))"
-      "l2h = (YulVariableDeclarationStatement (YulVariableDeclaration decls2 v2))"
-      "alpha_equiv_check_decls l1t l2t = Some (vs', fs)"
-      "vs = ((zip (map (\<lambda> x . case x of (YulTypedName n _) \<Rightarrow> n) decls1)
-                  (map (\<lambda> x . case x of (YulTypedName n _) \<Rightarrow> n) decls2)) @ vs')" |
-    (3) l1h l1t l2h l2t fs vs name1 args1 rets1 body1 name2 args2 rets2 body2 fs' where
-      "(locs', funcs') = (vs, fs)"
-      "sts1h#sts1t  = l1h # l1t"
-      "sts2 = l2h # l2t"
-      "yul_statement_same_constructor l1h l2h"
-      "l1h = (YulFunctionDefinitionStatement (YulFunctionDefinition name1 args1 rets1 body1))"
-      "l2h = (YulFunctionDefinitionStatement (YulFunctionDefinition name2 args2 rets2 body2))"
-      "alpha_equiv_check_decls l1t l2t = Some (vs, fs')"
-      "fs = (name1, name2)#fs'" |
-    (4) l1h l1t l2h l2t fs vs where
-    "(locs', funcs') = (vs, fs)"
-     "sts1h#sts1t  = l1h # l1t"
-     "sts2 = l2h # l2t"
-     "yul_statement_same_constructor l1h l2h"
-    "(case l1h of
-        YulVariableDeclarationStatement _ \<Rightarrow> False
-        | YulFunctionDefinitionStatement _ \<Rightarrow> False
-        | _ \<Rightarrow> True)"
-    "(case l2h of
-        YulVariableDeclarationStatement _ \<Rightarrow> False
-        | YulFunctionDefinitionStatement _ \<Rightarrow> False
-        | _ \<Rightarrow> True)"
-    "alpha_equiv_check_decls l1t l2t = Some (locs', funcs')"
-    using alpha_equiv_check_decls_cases_alt[OF Cons1.prems(1)] unfolding Cons2
-    by(clarsimp; metis)
-
-  then show ?case
-  proof cases
-    case 1
-    then show ?thesis by auto
-  next
-    case 2
-
-    have Arg : "alpha_equiv_check_decls sts1t l2t = Some (vs', fs)"
-      using Cons1.prems 2
-      by(auto)
-
-    show ?thesis using Cons1.prems Cons1.IH[OF Arg] Cons2 2
-      by(auto simp add: split: if_split_asm prod.splits)
-  next
-    case 3
-
-    have Arg : "alpha_equiv_check_decls sts1t l2t = Some (vs, fs')"
-      using Cons1.prems 3
-      by(auto)
-
-    show ?thesis using Cons1.prems Cons1.IH[OF Arg] Cons2 3
-      by(auto simp add: split: if_split_asm prod.splits)
-  next
-    case 4
-
-    have Arg : "alpha_equiv_check_decls sts1t l2t = Some (vs, fs)"
-      using Cons1.prems 4
-      by(auto)
-
-    show ?thesis using Cons1.prems Cons1.IH[OF Arg] Cons2 4
-      apply(cases l1h)
-                apply(cases l2h; auto)
-               apply(cases l2h; auto)
-              apply(cases l2h; auto)
-             apply(cases l2h; auto)
-            apply(cases l2h; auto)
-           apply(cases l2h; auto)
-          apply(cases l2h; auto)
-         apply(cases l2h; auto)
-      apply(cases l2h; auto)
-      apply(cases l2h; auto)
-      apply(cases l2h; auto)
-      done
-  qed
-qed
-  
-
-(* NB we are using combine_keep to avoid making
-changes to names field of existing functions.
-we actually know that there are no conflicts.
-
-induction on number of function decls in sts.
-*) 
-(*declare [[show_types]]*)
-
-lemma alpha_equiv_expr_fun_empty_2clause :
-  fixes x1 :: "(String.literal, 'a, 'b) YulFunctionCall'"
-  fixes st1 :: "(String.literal, 'a, 'b) YulExpression'"
-  shows "(\<forall> vsubst fsubst x2 f1 es1 f2 es2 . 
-          alpha_equiv_expr' vsubst fsubst (YulFunctionCallExpression x1) (YulFunctionCallExpression x2) \<longrightarrow>
-          x1 = (YulFunctionCall f1 es1) \<longrightarrow>
-          x2 = (YulFunctionCall f2 es2) \<longrightarrow> 
-      alpha_equiv_name' ([] # fsubst) f1 f2 \<and> list_all2 (alpha_equiv_expr' vsubst ([] # fsubst)) es1 es2)
-    \<and> (\<forall> vsubst fsubst st2 . alpha_equiv_expr' vsubst fsubst st1 st2 \<longrightarrow> alpha_equiv_expr' vsubst ([] # fsubst) st1 st2)"
-proof(induction rule: YulFunctionCall'_YulExpression'.induct)
-
-  case H : (YulFunctionCall x1 x2)
-  hence H' : "(\<And>x2a::(String.literal, 'a, 'b) YulExpression'.
-           x2a \<in> set x2 \<Longrightarrow>
-           (\<And>(vsubst::(String.literal \<times> String.literal) list list) (fsubst::(String.literal \<times> String.literal) list list)
-              st2::(String.literal, 'a, 'b) YulExpression'. alpha_equiv_expr' vsubst fsubst x2a st2 \<Longrightarrow> alpha_equiv_expr' vsubst ([] # fsubst) x2a st2))"
-    by blast
-
-  have Conc' : 
-"\<And> (vsubst::(String.literal \<times> String.literal) list list) (fsubst::(String.literal \<times> String.literal) list list)
-          (x2a::(String.literal, 'a, 'b) YulFunctionCall') (f1::String.literal) (es1::(String.literal, 'a, 'b) YulExpression' list) (f2::String.literal)
-          es2::(String.literal, 'a, 'b) YulExpression' list.
-          alpha_equiv_expr' vsubst fsubst (YulFunctionCallExpression (YulFunctionCall x1 x2)) (YulFunctionCallExpression x2a) \<Longrightarrow>
-          YulFunctionCall x1 x2 = YulFunctionCall f1 es1 \<Longrightarrow>
-          x2a = YulFunctionCall f2 es2 \<Longrightarrow> alpha_equiv_name' ([] # fsubst) f1 f2 \<and> list_all2 (alpha_equiv_expr' vsubst ([] # fsubst)) es1 es2"
-  proof-
-    fix vsubst fsubst x2a f1 es1 f2 es2
-
-    assume Hi1 : "alpha_equiv_expr' vsubst fsubst (YulFunctionCallExpression (YulFunctionCall x1 x2)) (YulFunctionCallExpression x2a)"
-    assume Hi2 : "YulFunctionCall x1 x2 = YulFunctionCall f1 es1"
-    assume Hi3 : "x2a = YulFunctionCall f2 es2" 
-
-    have Subexps : "list_all2 (alpha_equiv_expr' vsubst ([] # fsubst)) es1 es2"
-    proof(rule list_all2I)
-      show "\<forall>x\<in>set (zip es1 es2).
-       case x of (x, xa) \<Rightarrow> alpha_equiv_expr' vsubst ([] # fsubst) x xa"
-      proof
-        fix y
-        assume Y: "y \<in> set (zip es1 es2)"
-        
-        obtain y1 y2 where Y' : "y = (y1, y2)"
-          by(cases y; auto)
-
-        have Y1 : "y1 \<in> set es1" using set_zip_leftD[OF Y[unfolded Y']] 
-          by auto
-
-        have Y2 : "y2 \<in> set es2" using set_zip_rightD[OF Y[unfolded Y']] 
-          by auto
-
-        have X2eq : "es1 = x2" using Hi2 by auto
-
-        have Subs : "list_all2 (alpha_equiv_expr' vsubst fsubst) es1 es2"
-          using Hi1 Hi2 Hi3 Y'
-          by(auto simp add: )
-
-        then have Y_equiv : "(alpha_equiv_expr' vsubst (fsubst)) y1 y2"
-          using Y' Y
-          unfolding list_all2_iff
-          by(auto simp add: )
-
-        show "case y of (x, xa) \<Rightarrow> alpha_equiv_expr' vsubst ([] # fsubst) x xa"
-          using H'[OF Y1[unfolded X2eq] Y_equiv] Y'
-          by auto
-      qed
-    next
-      show "length es1 = length es2"
-        using Hi1 Hi2 Hi3 List.list_all2_lengthD
-        by(auto)
-    qed
-
-    show "alpha_equiv_name' ([] # fsubst) f1 f2 \<and> list_all2 (alpha_equiv_expr' vsubst ([] # fsubst)) es1 es2"
-      using H' Hi1 Hi2 Hi3 Subexps
-      by(auto simp add: alpha_equiv_name'_def)
-  qed
-  then show " \<forall>(vsubst::(String.literal \<times> String.literal) list list) (fsubst::(String.literal \<times> String.literal) list list)
-          (x2a::(String.literal, 'a, 'b) YulFunctionCall') (f1::String.literal) (es1::(String.literal, 'a, 'b) YulExpression' list) (f2::String.literal)
-          es2::(String.literal, 'a, 'b) YulExpression' list.
-          alpha_equiv_expr' vsubst fsubst (YulFunctionCallExpression (YulFunctionCall x1 x2)) (YulFunctionCallExpression x2a) \<longrightarrow>
-          YulFunctionCall x1 x2 = YulFunctionCall f1 es1 \<longrightarrow>
-          x2a = YulFunctionCall f2 es2 \<longrightarrow> alpha_equiv_name' ([] # fsubst) f1 f2 \<and> list_all2 (alpha_equiv_expr' vsubst ([] # fsubst)) es1 es2"
-    by blast
-next
-  case H: (YulFunctionCallExpression x)
-
-  have H' : "\<And> vsubst fsubst (x2 :: (String.literal, 'a, 'b) YulFunctionCall') f1 es1 f2 es2.
-     alpha_equiv_expr' vsubst fsubst (YulFunctionCallExpression x) (YulFunctionCallExpression x2) \<Longrightarrow>
-     x = YulFunctionCall f1 es1 \<Longrightarrow>
-     x2 = YulFunctionCall f2 es2 \<Longrightarrow> alpha_equiv_name' ([] # fsubst) f1 f2 \<and> list_all2 (alpha_equiv_expr' vsubst ([] # fsubst)) es1 es2"
-  proof-
-    fix x2 :: "((String.literal, 'a, 'b) YulFunctionCall')"
-    fix vsubst fsubst f1 es1 f2 es2
-    assume Hi1 : "alpha_equiv_expr' vsubst fsubst (YulFunctionCallExpression x) (YulFunctionCallExpression x2)"
-    assume Hi2 : "x = YulFunctionCall f1 es1"
-    assume Hi3 : "x2 = YulFunctionCall f2 es2" 
-    show "alpha_equiv_name' ([] # fsubst) f1 f2 \<and> list_all2 (alpha_equiv_expr' vsubst ([] # fsubst)) es1 es2"
-      using H Hi1 Hi2 Hi3
-      by(blast)
-  qed
-  have Conc' : "\<And>vsubst fsubst (st2 :: (String.literal, 'a, 'b) YulExpression').
-       alpha_equiv_expr' vsubst fsubst (YulFunctionCallExpression x) st2 \<Longrightarrow>
-       alpha_equiv_expr' vsubst ([] # fsubst) (YulFunctionCallExpression x) st2"
-  proof-
-    fix vsubst fsubst st2
-    assume Hi : "alpha_equiv_expr' vsubst fsubst (YulFunctionCallExpression x) st2"
-
-    obtain x2 where X2 : "st2 = YulFunctionCallExpression x2"
-      using Hi by (cases st2; auto)
-
-    obtain f1 es1 where Xc : "x = YulFunctionCall f1 es1"
-      by(cases x; auto)
-
-    obtain f2 es2 where Xc2 : "x2 = YulFunctionCall f2 es2"
-      by(cases x2; auto)
-
-    show "alpha_equiv_expr' vsubst ([] # fsubst) (YulFunctionCallExpression x) st2"
-      using H'[OF Hi[unfolded X2] Xc Xc2] X2 Xc Xc2
-      by(auto simp add: alpha_equiv_name'_def)
-  qed
-
-  then show ?case
-    by blast
-next
-  case H : (YulIdentifier x)
-
-  have Conc' : "\<And> vsubst fsubst (st2 :: (String.literal, 'a, 'b) YulExpression').
-            alpha_equiv_expr' vsubst fsubst (YulIdentifier x) st2 \<Longrightarrow>
-            alpha_equiv_expr' vsubst ([] # fsubst) (YulIdentifier x) st2"
-  proof-
-    fix st2 :: "(String.literal, 'a, 'b) YulExpression'"
-    fix vsubst fsubst
-    assume "alpha_equiv_expr' vsubst fsubst (YulIdentifier x) st2"
-    then show "alpha_equiv_expr' vsubst ([] # fsubst) (YulIdentifier x) st2"
-      by(cases st2; auto )
-  qed
-  then show ?case by blast
-next
-  case H : (YulLiteralExpression x)
-  have Conc' : "\<And> vsubst fsubst (st2 :: (String.literal, 'a, 'b) YulExpression').
-            alpha_equiv_expr' vsubst fsubst (YulLiteralExpression x) st2 \<Longrightarrow>
-            alpha_equiv_expr' vsubst ([] # fsubst) (YulLiteralExpression x) st2"
-  proof-
-    fix st2 :: "(String.literal, 'a, 'b) YulExpression'"
-    fix vsubst fsubst
-    assume "alpha_equiv_expr' vsubst fsubst (YulLiteralExpression x) st2"
-    then show "alpha_equiv_expr' vsubst ([] # fsubst) (YulLiteralExpression x) st2"
-      by(cases st2; auto )
-  qed
-  then show ?case by blast
-qed
-
-(* YOU ARE HERE.
- * either need alpha equiv for switch cases,
- * or otherwise rewrite the second clause *)
-lemma alpha_equiv_expr_fun_empty :
-  assumes "alpha_equiv_expr' vsubst fsubst st1 st2"
-  shows "alpha_equiv_expr' vsubst ([] # fsubst) st1 st2"
-  using assms alpha_equiv_expr_fun_empty_2clause
-  by blast
-term "YulFunctionDefinition"
-lemma alpha_equiv_statement_fun_empty' :
-  fixes st1 :: "(String.literal, 'a, 'b) YulStatement'"
-  fixes sc :: "(String.literal, 'a, 'b) YulSwitchCase'"
-  fixes fd :: "(String.literal, 'a, 'b) YulFunctionDefinition'"
-  shows "(\<forall> vsubst fsubst st2 . alpha_equiv_statement' vsubst fsubst st1 st2 \<longrightarrow> alpha_equiv_statement' vsubst ([] # fsubst) st1 st2) \<and>
-         (\<forall> vsubst fsubst lit sts sts2 sc2 e1 e2 . sc = YulSwitchCase lit sts \<longrightarrow> list_all2 (alpha_equiv_statement' vsubst fsubst) sts sts2 \<longrightarrow>
-            list_all2 (alpha_equiv_statement' vsubst fsubst) sts sts2) \<and>
-         (\<forall> vsubst fsubst st2 . alpha_equiv_statement' vsubst fsubst (YulFunctionDefinitionStatement fd) st2 \<longrightarrow> alpha_equiv_statement' vsubst ([] # fsubst) (YulFunctionDefinitionStatement fd) st2)"
-proof(induction  rule: YulStatement'_YulSwitchCase'_YulFunctionDefinition'.induct)
-  case C: (YulFunctionCallStatement x)
-
-  obtain a b where AB: "x =  YulFunctionCall a b"
-    by(cases x; auto)
-
-  have Conc' : "\<And> vsubst fsubst st2.
-            alpha_equiv_statement' vsubst fsubst (YulFunctionCallStatement x)
-             st2 \<Longrightarrow>
-            alpha_equiv_statement' vsubst ([] # fsubst)
-             (YulFunctionCallStatement x) st2"
-  proof-
-    fix vsubst fsubst
-    fix st2 :: "(String.literal, 'a, 'b) YulStatement'"
-
-    assume H: "alpha_equiv_statement' vsubst fsubst (YulFunctionCallStatement x) st2"
-
-    obtain x2 where X2: "st2 = YulFunctionCallStatement x2"
-      using H AB
-      by(cases st2; auto)
-
-    then obtain f g where FG : "x2 = YulFunctionCall f g"
-      by(cases x2; auto)
-
-    have Final : "list_all2 (alpha_equiv_expr' vsubst ([] # fsubst)) b g"
-    proof(rule list_all2I)
-      show "\<forall>x\<in>set (zip b g).
-       case x of (x, xa) \<Rightarrow> alpha_equiv_expr' vsubst ([] # fsubst) x xa"
-      proof
-        fix w
-        assume W: "w \<in> set (zip b g)"
-
-        obtain w1 w2 where W' : "w = (w1, w2)"
-          by(cases w; auto)
-
-        have W1 : "w1 \<in> set b" using set_zip_leftD[OF W[unfolded W']] 
-          by auto
-
-        have W2 : "w2 \<in> set g" using set_zip_rightD[OF W[unfolded W']] 
-          by auto
-
-        have Subs : "list_all2 (alpha_equiv_expr' vsubst fsubst) b g"
-          using AB H X2 FG W'
-          by(auto simp add: )
-
-        then have W_equiv : "(alpha_equiv_expr' vsubst (fsubst)) w1 w2"
-          using W' W
-          unfolding list_all2_iff
-          by(auto simp add: )
-
-        show "case w of (x, xa) \<Rightarrow> alpha_equiv_expr' vsubst ([] # fsubst) x xa"
-          using alpha_equiv_expr_fun_empty[OF W_equiv] W'
-          by auto
-      qed
-    next
-      show "length b = length g"
-        using AB H X2 FG List.list_all2_lengthD
-        by(auto)
-    qed
-
-    then show "alpha_equiv_statement' vsubst ([] # fsubst) (YulFunctionCallStatement x)
-        st2" using AB X2 H FG
-      by(auto)
-  qed
-
-  then show ?case by blast
-next
-  case C: (YulAssignmentStatement x)
-
-  obtain a b where AB: "x =  YulAssignment a b"
-    by(cases x; auto)
-
-  have Conc' : "\<And> vsubst fsubst st2.
-            alpha_equiv_statement' vsubst fsubst (YulAssignmentStatement x)
-             st2 \<Longrightarrow>
-            alpha_equiv_statement' vsubst ([] # fsubst)
-             (YulAssignmentStatement x) st2"
-  proof-
-    fix vsubst fsubst
-    fix st2 :: "(String.literal, 'a, 'b) YulStatement'"
-
-    assume H: "alpha_equiv_statement' vsubst fsubst (YulAssignmentStatement x) st2"
-
-    obtain x2 where X2: "st2 = YulAssignmentStatement x2"
-      using H AB
-      by(cases st2; auto)
-
-    then obtain f g where FG : "x2 = YulAssignment f g"
-      by(cases x2; auto)
-
-    have Subs : " (alpha_equiv_expr' vsubst fsubst) b g"
-      using AB H X2 FG
-      by(auto simp add: )
-
-    then have Final : "(alpha_equiv_expr' vsubst ([] # fsubst)) b g"
-      using alpha_equiv_expr_fun_empty[OF Subs]
-      by auto
-
-    then show "alpha_equiv_statement' vsubst ([] # fsubst) (YulAssignmentStatement x)
-        st2" using AB X2 H FG
-      by(auto)
-  qed
-
-  then show ?case by blast
-next
-  case C: (YulVariableDeclarationStatement x)
-
-  obtain a b where AB: "x =  YulVariableDeclaration a b"
-    by(cases x; auto)
-
-  have Conc' : "\<And> vsubst fsubst st2.
-            alpha_equiv_statement' vsubst fsubst (YulVariableDeclarationStatement x)
-             st2 \<Longrightarrow>
-            alpha_equiv_statement' vsubst ([] # fsubst)
-             (YulVariableDeclarationStatement x) st2"
-  proof-
-    fix vsubst fsubst
-    fix st2 :: "(String.literal, 'a, 'b) YulStatement'"
-
-    assume H: "alpha_equiv_statement' vsubst fsubst (YulVariableDeclarationStatement x) st2"
-
-    obtain x2 where X2: "st2 = YulVariableDeclarationStatement x2"
-      using H AB
-      by(cases st2; auto)
-
-    then obtain f g where FG : "x2 = YulVariableDeclaration f g"
-      by(cases x2; auto)
-
-    show "alpha_equiv_statement' vsubst ([] # fsubst) (YulVariableDeclarationStatement x) st2"
-    proof(cases b)
-      case None
-      then show ?thesis using AB X2 H FG
-      by(auto)
-    next
-      case (Some b')
-
-      then obtain g' where Some' : "g = Some g'"
-        using H X2 FG AB
-        by(cases g; auto)
-
-      then show ?thesis
-        using H X2 FG AB Some alpha_equiv_expr_fun_empty
-        by(auto)
-    qed
-  qed
-  then show ?case by blast
-next
-
-  case C: (YulFunctionDefinitionStatement x)
-
-  obtain a b c d where AB: "x =  YulFunctionDefinition a b c d"
-    by(cases x; auto)
-
-  have Hyp' : "\<And> vsubst fsubst st2.
-            alpha_equiv_statement' vsubst fsubst
-             (YulFunctionDefinitionStatement x) st2 \<Longrightarrow>
-            alpha_equiv_statement' vsubst ([] # fsubst)
-             (YulFunctionDefinitionStatement x) st2 "
-    using C by blast
-
-  have Conc' : "\<And> vsubst fsubst st2.
-            alpha_equiv_statement' vsubst fsubst (YulFunctionDefinitionStatement x)
-             st2 \<Longrightarrow>
-            alpha_equiv_statement' vsubst ([] # fsubst)
-             (YulFunctionDefinitionStatement x) st2"
-  proof-
-    fix vsubst fsubst
-    fix st2 :: "(String.literal, 'a, 'b) YulStatement'"
-
-    assume H: "alpha_equiv_statement' vsubst fsubst (YulFunctionDefinitionStatement x) st2"
-
-    obtain x2 where X2: "st2 = YulFunctionDefinitionStatement x2"
-      using H AB
-      by(cases st2; auto)
-
-    then obtain f g h i where FG : "x2 = YulFunctionDefinition f g h i"
-      by(cases x2; auto)
-
-    show "alpha_equiv_statement' vsubst ([] # fsubst) (YulFunctionDefinitionStatement x) st2"
-      using Hyp'[OF H]
-      by auto
-  qed
-  then show ?case by blast
-next
-  case C: (YulIf x1 x2)
-
-  have Hyp' : "\<And> s . s \<in> set x2 \<Longrightarrow>
-    (\<And> vsubst fsubst st2.
-     alpha_equiv_statement' vsubst fsubst s st2 \<longrightarrow>
-     alpha_equiv_statement' vsubst ([] # fsubst) s st2)"
-    using C by blast
-
-  have Conc' : "\<And> vsubst fsubst st2.
-          alpha_equiv_statement' vsubst fsubst (YulIf x1 x2) st2 \<Longrightarrow>
-          alpha_equiv_statement' vsubst ([] # fsubst) (YulIf x1 x2) st2"
-  proof-
-    fix vsubst fsubst
-    fix vsubst fsubst
-    fix st2 :: "(String.literal, 'a, 'b) YulStatement'"
-
-    assume H: "alpha_equiv_statement' vsubst fsubst (YulIf x1 x2) st2"
-
-    obtain y1 y2 where Y: "st2 = YulIf y1 y2"
-      using H
-      by(cases st2; auto)
-
-    have E : "alpha_equiv_expr' vsubst ([] # fsubst) x1 y1" 
-      using H Y alpha_equiv_expr_fun_empty
-      by(auto)
-
-    obtain locs funcs where Decls : "alpha_equiv_check_decls x2 y2 = Some (locs, funcs)"
-      using H Y
-      by(auto split: option.split_asm)
-
-    show "alpha_equiv_statement' vsubst ([] # fsubst) (YulIf x1 x2) st2"
-      using Hyp' Y E Decls
-      apply auto    
-    sorry
-
-  then show ?case by blast
-next
-  case (YulSwitch x1 x2)
-  then show ?case sorry
-next
-  case (YulForLoop x1 x2 x3 x4)
-then show ?case sorry
-next
-  case YulBreak
-then show ?case sorry
-next
-  case YulContinue
-  then show ?case sorry
-next
-  case YulLeave
-  then show ?case sorry
-next
-case (YulBlock x)
-  then show ?case sorry
-next
-case (YulSwitchCase x1 x2)
-  then show ?case sorry
-next
-case (YulFunctionDefinition x1 x2 x3 x4)
-  then show ?case sorry
-qed
-
-  case (YulFunctionDefinitionStatement x)
-  then show ?thesis sorry
-next
-  case (YulIf x51 x52)
-  then show ?thesis sorry
-next
-  case (YulSwitch x61 x62)
-  then show ?thesis sorry
-next
-  case (YulForLoop x71 x72 x73 x74)
-  then show ?thesis sorry
-next
-  case YulBreak
-  then show ?thesis sorry
-next
-  case YulContinue
-  then show ?thesis sorry
-next
-  case YulLeave
-  then show ?thesis sorry
-next
-  case (YulBlock x11)
-  then show ?thesis sorry
-qed
-
-
-(* need a version of this for statements. *)
-lemma alpha_equiv_fun_empty :
-  assumes H: "alpha_equiv_fun vsubst fsubst f1 f2"
-  shows "alpha_equiv_fun vsubst ([]#fsubst) f1 f2"
-  using H
-proof(induction fsubst arbitrary: vsubst)
-  case Nil
-
-  obtain n1 s1 where F1 : "f1 = (n1, s1)"
-    by(cases f1; auto)
-
-  obtain n2 s2 where F2 : "f2 = (n2, s2)"
-    by(cases f2; auto)
-
-  show ?case
-  proof(cases "f_sig_body s1")
-    case (YulBuiltin x1)
-    then show ?thesis using Nil F1 F2
-    by(auto simp add: alpha_equiv_fun_def alpha_equiv_function_sig'_scheme_def)
-  next
-    case X1 : (YulFunction x1)
-
-    obtain x2 where X2 : "f_sig_body s2 = YulFunction x2"
-      using Nil X1 F1 F2
-      by(cases "f_sig_body s2"; auto simp add: alpha_equiv_fun_def alpha_equiv_function_sig'_scheme_def)
-
-(* alpha_equiv_statement'_nil - adding nil on the end has no effect *)
-    then show ?thesis using Nil F1 F2 X1 X2 list_all2_map
-      apply(auto simp add: alpha_equiv_fun_def alpha_equiv_function_sig'_scheme_def
-split: option.splits) 
-      sorry
-  qed
-next
-  case (Cons fh ft)
-
-  obtain n1 s1 where F1 : "f1 = (n1, s1)"
-    by(cases f1; auto)
-
-  obtain n2 s2 where F2 : "f2 = (n2, s2)"
-    by(cases f2; auto)
-
-  show ?case
-  proof(cases "f_sig_body s1")
-    case (YulBuiltin x1)
-    then show ?thesis using Cons.prems F1 F2
-    by(auto simp add: alpha_equiv_fun_def alpha_equiv_function_sig'_scheme_def)
-  next
-    case X1 : (YulFunction x1)
-
-    obtain x2 where X2 : "f_sig_body s2 = YulFunction x2"
-      using Cons.prems X1 F1 F2
-      by(cases "f_sig_body s2"; auto simp add: alpha_equiv_fun_def alpha_equiv_function_sig'_scheme_def)
-
-(* alpha_equiv_statement'_nil - adding nil on the end has no effect *)
-    then show ?thesis using Cons F1 F2 X1 X2
-      apply(auto simp add: alpha_equiv_fun_def alpha_equiv_function_sig'_scheme_def
-split: option.splits) 
-      sorry
-  qed
-
-  then show ?case
-    apply(auto simp add: alpha_equiv_fun_def alpha_equiv_function_sig'_scheme_def)
-qed
-
-lemma alpha_equiv_gather_funs'_combine :
-  assumes Decls : "alpha_equiv_check_decls (pre1 @ sts1) (pre2 @ sts2) = Some (locs', funcs')"
-  assumes Equiv : "alpha_equiv_funs' vsubst' fsubst funs1 funs2"
-  assumes Sts : "list_all2 (alpha_equiv_statement' (locs' # vsubst') (funcs' # fsubst))
-     sts1 sts2"
-  assumes Gather1 :
-    "gatherYulFunctions' (map (\<lambda>(n, fs). (n, function_sig'.truncate fs)) funs1) sts1 =
-      Inl fs1"
-  assumes Gather2 :
-     "gatherYulFunctions' (map (\<lambda>(n, fs). (n, function_sig'.truncate fs)) funs2) sts2 =
-       Inl fs2"
-  shows "alpha_equiv_funs' vsubst' (zip (get_fun_decls sts1) (get_fun_decls sts2) # fsubst)
-     (combine_keep (funs1)
-       (map (\<lambda>(n, fs). (n, function_sig'.extend fs \<lparr>f_sig_visible = map fst fs1\<rparr>))
-         fs1))
-     (combine_keep (funs2)
-       (map (\<lambda>(n, fs). (n, function_sig'.extend fs \<lparr>f_sig_visible = map fst fs2\<rparr>))
-         fs2))"
-  using assms
-proof(induction sts1 arbitrary: pre1 pre2 sts2 locs' funcs' funs1 fs1 funs2 fs2 vsubst' fsubst)
-  case Nil1 : Nil
-
-  have Nil2 : "sts2 = []"
-    using Nil1
-    by(cases sts2; auto)
-
-  then show ?case using Nil1 alpha_equiv_funs_trunc[OF Nil1(2)]
-    apply(auto simp add: alpha_equiv_funs'_def alpha_equiv_fun_def)
-    sorry
-next
-  case Cons1 : (Cons h1 t1)
-
-  then obtain h2 t2 where Cons2 : "sts2 = h2#t2"
-    by(cases sts2; auto)
-
-  have Reassoc :
-    "alpha_equiv_check_decls ((pre1 @ [h1]) @ t1) ((pre2 @ [h2]) @ t2) = Some (locs', funcs')"
-    using Cons1.prems Cons2
-    by auto
-
-  have Eqv_tl :
-    "list_all2 (alpha_equiv_statement' (locs' # vsubst') (funcs' # fsubst)) t1 t2"
-    using Cons1.prems
-    unfolding Cons2
-    by(auto)
-
-  show ?case
-    using Cons1.IH[OF Reassoc Cons1.prems(2) Eqv_tl] Cons1.prems
-
-
-  consider 
-    (1) "(pre1 @ h1#t1 = [] \<and> pre2 @ sts2 = [] \<and> (locs', funcs') = ([], []))" |
-    (2) l1h l1t l2h l2t fs vs decls1 v1 decls2 v2 vs' where 
-      "(locs', funcs') = (vs, fs)"
-      "pre1 @ h1#t1 = l1h # l1t"
-      "pre2 @ sts2 = l2h # l2t"
-      "yul_statement_same_constructor l1h l2h"
-      "l1h = (YulVariableDeclarationStatement (YulVariableDeclaration decls1 v1))"
-      "l2h = (YulVariableDeclarationStatement (YulVariableDeclaration decls2 v2))"
-      "alpha_equiv_check_decls l1t l2t = Some (vs', fs)"
-      "vs = ((zip (map (\<lambda> x . case x of (YulTypedName n _) \<Rightarrow> n) decls1)
-                  (map (\<lambda> x . case x of (YulTypedName n _) \<Rightarrow> n) decls2)) @ vs')" |
-    (3) l1h l1t l2h l2t fs vs name1 args1 rets1 body1 name2 args2 rets2 body2 fs' where
-      "(locs', funcs') = (vs, fs)"
-      "pre1 @ h1#t1 = l1h # l1t"
-      "pre2 @ sts2 = l2h # l2t"
-      "yul_statement_same_constructor l1h l2h"
-      "l1h = (YulFunctionDefinitionStatement (YulFunctionDefinition name1 args1 rets1 body1))"
-      "l2h = (YulFunctionDefinitionStatement (YulFunctionDefinition name2 args2 rets2 body2))"
-      "alpha_equiv_check_decls l1t l2t = Some (vs, fs')"
-      "fs = (name1, name2)#fs'" |
-    (4) l1h l1t l2h l2t fs vs where
-    "(locs', funcs') = (vs, fs)"
-     "pre1 @ h1#t1 = l1h # l1t"
-     "pre2 @ sts2 = l2h # l2t"
-     "yul_statement_same_constructor l1h l2h"
-    "(case l1h of
-        YulVariableDeclarationStatement _ \<Rightarrow> False
-        | YulFunctionDefinitionStatement _ \<Rightarrow> False
-        | _ \<Rightarrow> True)"
-    "(case l2h of
-        YulVariableDeclarationStatement _ \<Rightarrow> False
-        | YulFunctionDefinitionStatement _ \<Rightarrow> False
-        | _ \<Rightarrow> True)"
-    "alpha_equiv_check_decls l1t l2t = Some (locs', funcs')"
-    using alpha_equiv_check_decls_cases_alt[OF Cons1.prems(1)] unfolding Cons2
-    by(auto)
-
-  then show ?case
-  proof cases
-    case 1
-    then show ?thesis using Cons1 by auto
-  next
-    case 2
-
-    have Eq0 : "locs' = vs" "funcs' = fs"
-      using 2 by auto
-
-    have Eq1 : "h1 = l1h" "t1 = l1t"
-      using 2 by auto
-
-    have Eq2 : "h2 = l2h" "t2 = l2t"
-      using 2 Cons2 by auto
-
-    have All_tl : "list_all2 (alpha_equiv_statement' (locs' # vsubst') (funcs' # fsubst)) (l1t) l2t"
-      using Cons1.prems Cons2 Eq0 Eq1 Eq2
-      by auto
-
-    show ?thesis 
-      using Cons1.IH[unfolded Cons2, unfolded Eq0, unfolded Eq1, unfolded Eq2
-                    , OF "2"(7) Cons1.prems(2)] Cons1.prems
-      using All_tl[unfolded Eq0]
-      using "2"(8)
-(* something related to extending locals environment...
-   relate decls to insert values? *)
-  next
-    case 3
-    then show ?thesis sorry
-  next
-    case 4
-    then show ?thesis sorry
-  qed
-
-(*
-"(l1 = [] \<and> l2 = [] \<and> x = ([], [])) \<or>
-     (\<exists> l1h l1t l2h l2t fs vs . x = (vs, fs) \<and>
-      l1 = l1h # l1t \<and> l2 = l2h # l2t \<and> yul_statement_same_constructor l1h l2h \<and> 
-      (\<exists> decls1 v1 decls2 v2 vs' .
-        l1h = (YulVariableDeclarationStatement (YulVariableDeclaration decls1 v1)) \<and>
-        l2h = (YulVariableDeclarationStatement (YulVariableDeclaration decls2 v2)) \<and>
-        alpha_equiv_check_decls l1t l2t = Some (vs', fs) \<and>
-        vs = ((zip (map (\<lambda> x . case x of (YulTypedName n _) \<Rightarrow> n) decls1)
-                   (map (\<lambda> x . case x of (YulTypedName n _) \<Rightarrow> n) decls2)) @ vs')) \<or>
-      (\<exists> name1 args1 rets1 body1 name2 args2 rets2 body2 fs' .
-        l1h = (YulFunctionDefinitionStatement (YulFunctionDefinition name1 args1 rets1 body1)) \<and>
-        l2h = (YulFunctionDefinitionStatement (YulFunctionDefinition name2 args2 rets2 body2)) \<and>
-        alpha_equiv_check_decls l1t l2t = Some (vs, fs') \<and>
-        fs = (name1, name2)#fs') \<or>
-      ((case l1h of
-        YulVariableDeclarationStatement _ \<Rightarrow> False
-        | YulFunctionDefinitionStatement _ \<Rightarrow> False
-        | _ \<Rightarrow> True) \<and>
-       (case l2h of
-        YulVariableDeclarationStatement _ \<Rightarrow> False
-        | YulFunctionDefinitionStatement _ \<Rightarrow> False
-        | _ \<Rightarrow> True) \<and> alpha_equiv_check_decls l1t l2t = Some x))"
-*)
-  obtain locs0 funcs0 locs1 funcs1 where
-    Split : "alpha_equiv_check_decls t1 t2 = Some (locs1, funcs1)"
-       "locs' = locs0 @ locs1" "funcs' = funcs0 @ funcs1"
-    sorry
-  show ?case using Cons1.IH[OF Split(1) Cons1.prems(2)] Cons1.prems(3) 
-    using Cons1.prems alpha_equiv_funs_trunc
-      apply(auto simp add: alpha_equiv_funs'_def alpha_equiv_fun_def 
-       get_fun_decls_def get_var_decls_def Let_def split:if_splits)
-    apply(clarsimp)
-*)
 
 lemma gatherYulFunctions'_notin :
   assumes "gatherYulFunctions' (map (\<lambda>(n, fs). (n, function_sig'.truncate fs)) (funs r1)) st1 =
@@ -2094,7 +922,7 @@ assumes Hg1 : "gatherYulFunctions'
   (map (\<lambda>(n, fs). (n, function_sig'.truncate fs)) (funs r1)) sts1 = Inl fs1"
 assumes Hg2 : "gatherYulFunctions'
    (map (\<lambda>(n, fs). (n, function_sig'.truncate fs)) (funs r2)) sts2 = Inl fs2"
-assumes Heqv :  "list_all2 (alpha_equiv_statement' ((pre @ funcs') # fsubst) False) sts1 sts2"
+assumes Heqv :  "list_all2 (alpha_equiv_statement' ((pre @ funcs') # fsubst)) sts1 sts2"
 assumes Hcheck : "alpha_equiv_check_decls sts1 sts2 = Some (funcs')"
 assumes Hpre1 : "distinct (map fst (pre @ funcs'))"
 assumes Hpre2 : "distinct (map snd (pre @ funcs'))"
@@ -2213,7 +1041,7 @@ next
         Gather1_None Gather2_None Funs1_None Noshadow'
       by (cases "map_of (subst'_flip funs_t) n1"; auto)
 
-    have Eqv' : "list_all2 (alpha_equiv_statement' (((pre @ [(n1, n2)]) @ funs_t) # fsubst) False) stt1 stt2"
+    have Eqv' : "list_all2 (alpha_equiv_statement' (((pre @ [(n1, n2)]) @ funs_t) # fsubst)) stt1 stt2"
       using Cons1.prems Cons2 X4 Y4 F1 F2 Funs_t Funs_body Gather1 Gather2 
         Gather1_None Gather2_None Funs1_None Funs2_None Noshadow' Noshadow_flip2
       by(auto)
@@ -2485,7 +1313,7 @@ assumes Hg1 : "gatherYulFunctions'
   (map (\<lambda>(n, fs). (n, function_sig'.truncate fs)) (funs r1)) sts1 = Inl fs1"
 assumes Hg2 : "gatherYulFunctions'
    (map (\<lambda>(n, fs). (n, function_sig'.truncate fs)) (funs r2)) sts2 = Inl fs2"
-assumes Heqv :  "list_all2 (alpha_equiv_statement' ((pre @ funcs') # fsubst) False) sts1 sts2"
+assumes Heqv :  "list_all2 (alpha_equiv_statement' ((pre @ funcs') # fsubst)) sts1 sts2"
 assumes Hcheck : "alpha_equiv_check_decls sts1 sts2 = Some (funcs')"
 assumes Hpre1 : "distinct (map fst (pre @ funcs'))"
 assumes Hpre2 : "distinct (map snd (pre @ funcs'))"
@@ -2603,7 +1431,7 @@ next
         Gather1_None Gather2_None Funs1_None Funs2_None Noshadow Noshadow_flip2
       by(auto)
 
-    have Eqv' : "list_all2 (alpha_equiv_statement' (((pre @ [(n1, n2)]) @ funs_t) # fsubst) False) stt1 stt2"
+    have Eqv' : "list_all2 (alpha_equiv_statement' (((pre @ [(n1, n2)]) @ funs_t) # fsubst)) stt1 stt2"
       using Cons1.prems Cons2 X4 Y4 F1 F2 Funs_t Funs_body Gather1 Gather2 
         Gather1_None Gather2_None Funs1_None Funs2_None Noshadow' Noshadow_flip2
       by(auto)
@@ -2983,6 +1811,67 @@ next
 qed
 *)
 
+lemma alpha_equiv_locals'_eq :
+  shows "alpha_equiv_locals' fsubst x x"
+proof(induction x arbitrary: fsubst)
+  case Nil
+  then show ?case
+    by(auto simp add: alpha_equiv_locals'_def)
+next
+  case (Cons xh xt)
+  then show ?case
+    by(auto simp add: alpha_equiv_locals'_def)
+qed
+
+(*lemma*)
+
+lemma alpha_equiv_stackEls'_enter :
+  assumes "list_all2 (alpha_equiv_statement' subst) sts1 sts2"
+  shows
+    "alpha_equiv_stackEls'
+     (subst)
+     (map EnterStatement sts1) (map EnterStatement sts2)"
+  using assms
+proof(induction sts1 arbitrary: subst sts2)
+  case Nil
+  then show ?case 
+    by(auto)
+next
+  case Cons1 : (Cons st1h st1t)
+
+  obtain st2h st2t where Cons2 :
+    "sts2 = st2h # st2t"
+    using Cons1.prems
+    by(cases sts2; auto)
+
+  show ?case using Cons1 Cons2
+    by(cases st1h; cases st2h; auto)
+qed
+
+lemma alpha_equiv_stackEls'_newsubst_enter :
+  assumes "list_all2 (alpha_equiv_statement' subst) sts1 sts2"
+  shows
+    "alpha_equiv_stackEls'_newsubst
+     (subst)
+     (map EnterStatement sts1) (map EnterStatement sts2) = Some subst"
+  using assms
+proof(induction sts1 arbitrary: subst sts2)
+  case Nil
+  then show ?case 
+    by(auto)
+next
+  case Cons1 : (Cons st1h st1t)
+
+  obtain st2h st2t where Cons2 :
+    "sts2 = st2h # st2t"
+    using Cons1.prems
+    by(cases sts2; auto)
+
+  show ?case using Cons1 Cons2
+    by(cases st1h; cases st2h; auto)
+qed
+
+
 (* YOU ARE HERE. See if we still need the check_decls cases lemma. *)
 lemma alpha_equiv_step :
   assumes Hc1 : "cont r1 = (c1h#c1t)"
@@ -3017,11 +1906,10 @@ proof(cases c1h)
       FC2 : "f2 = YulFunctionCall n2 args2"
       by(cases f2; auto)
 
-    show ?thesis 
+    show ?thesis
       using ES1 F1 FC1 ES2 F2 FC2 Hinit H1 H2 Hc1 Hc2 Hupd
       by(auto simp add: alpha_equiv_results'_def alpha_equiv_locals'_def)
   next
-
     case A1 : (YulAssignmentStatement a1)
 
     then obtain vs1 e1 where
@@ -3197,10 +2085,11 @@ proof(cases c1h)
       using alpha_equiv_gather_functions[OF Fs1 Fs2 _ Decls, of "[]" fsubst]
       by(auto simp add: alpha_equiv_results'_def alpha_equiv_funs'_def)
 
+
 (* statement equivalence implies stackEl equivalence for enter statement
  * statement equivalence, locals equality, funs equivalence
  * implies stackel equivalence for exit statement *)
-
+(*
     have Conc2 : "list_all2 (alpha_equiv_stackEl' (zip (get_fun_decls sts1) (get_fun_decls sts2) # fsubst))
      (map EnterStatement sts1 @ ExitStatement (YulBlock sts1) (locals r2) (funs r1) # c1t)
      (map EnterStatement sts2 @ ExitStatement (YulBlock sts2) (locals r2) (funs r2) # c2t)"
@@ -3239,6 +2128,7 @@ proof(cases c1h)
 
       qed
 
+
       then show "list_all2
        (alpha_equiv_stackEl'
          (zip (get_fun_decls sts1) (get_fun_decls sts2) # fsubst))
@@ -3246,45 +2136,55 @@ proof(cases c1h)
        (ExitStatement (YulBlock sts2) (locals r2) (funs r2) # c2t)"
         by simp
     qed
+*)
+
+(* this is promising.
+ * we just need:
+ * - admitted lemmas above about splitting equiv_stackEls'
+ * - lemma saying that comparing map EnterStatement for equality is just
+ *   comparing statements for equality
+ * - lemma saying that EnterStatement doesn't
+     affect the substitution
+ *)
+    have Conc2 :
+      "alpha_equiv_stackEls' (zip (get_fun_decls sts1) (get_fun_decls sts2) # fsubst)
+       (map EnterStatement sts1 @ ExitStatement (YulBlock sts1) (locals r2) (funs r1) # c1t)
+       (map EnterStatement sts2 @ ExitStatement (YulBlock sts2) (locals r2) (funs r2) # c2t)"
+    proof(rule alpha_equiv_stackEls'_split)
+      show "alpha_equiv_stackEls'
+       (zip (get_fun_decls sts1)
+         (get_fun_decls sts2) #
+        fsubst)
+       (map EnterStatement sts1)
+       (map EnterStatement sts2)"
+        using ES1 B1 ES2 B2 Hinit H1 H2 Hc1 Hc2 Hupd Fs1 Fs2 Decls Decls_eq
+        using alpha_equiv_stackEls'_enter
+        unfolding alpha_equiv_results'_def
+        by(auto simp add: alpha_equiv_results'_def alpha_equiv_funs'_def alpha_equiv_locals'_eq)
+    next
+      show "alpha_equiv_stackEls'_newsubst
+           (zip (get_fun_decls sts1) (get_fun_decls sts2) # fsubst)
+           (map EnterStatement sts1) (map EnterStatement sts2) =
+          Some (zip (get_fun_decls sts1) (get_fun_decls sts2) # fsubst)"
+        using ES1 B1 ES2 B2 Hinit H1 H2 Hc1 Hc2 Hupd Fs1 Fs2 Decls Decls_eq
+        using alpha_equiv_stackEls'_newsubst_enter
+        unfolding alpha_equiv_results'_def
+        by(auto simp add: alpha_equiv_results'_def alpha_equiv_funs'_def alpha_equiv_locals'_eq)
+    next
+      show "alpha_equiv_stackEls'
+     (zip (get_fun_decls sts1) (get_fun_decls sts2) # fsubst)
+     (ExitStatement (YulBlock sts1) (locals r2) (funs r1) # c1t)
+     (ExitStatement (YulBlock sts2) (locals r2) (funs r2) # c2t)"
+        using ES1 B1 ES2 B2 Hinit H1 H2 Hc1 Hc2 Hupd Fs1 Fs2 Decls Decls_eq
+        unfolding alpha_equiv_results'_def
+        by(auto simp add: alpha_equiv_results'_def alpha_equiv_funs'_def alpha_equiv_locals'_eq)
+    qed
+
     show ?thesis
       using ES1 B1 ES2 B2 Hinit H1 H2 Hc1 Hc2 Hupd Fs1 Fs2 Decls Conc1 Conc2
       unfolding alpha_equiv_results'_def
       by(auto simp add: alpha_equiv_results'_def alpha_equiv_funs'_def)
-
-(*
-assumes Heqv : "alpha_equiv_check_decls sts1 sts2 = Some funcs'"
-assumes Hsts : "list_all2 (alpha_equiv_statement' (funcs' # fsubst)) sts1 sts2"
-assumes Hfuns : "list_all2 (alpha_equiv_fun fsubst) (funs r1) (funs r2)"
-assumes Htail : "list_all2 (alpha_equiv_stackEl' fsubst) c1t c2t"
-shows
-  "list_all2
-    (alpha_equiv_stackEl'
-      (zip (get_fun_decls sts1) (get_fun_decls sts2) # fsubst))
-    (map EnterStatement sts1 @
-     ExitStatement (YulBlock sts1) (locals r2) (funs r1) # c1t)
-    (map EnterStatement sts2 @
-     ExitStatement (YulBlock sts2) (locals r2) (funs r2) # c2t)"
-
-      then show ?thesis sorry
-*)
-(*
-gatherYulFunctions'
- (map (\<lambda>(n, fs). (n, function_sig'.truncate fs)) (funs r1)) sts1 = Inl fs1 \<Longrightarrow>
-gatherYulFunctions'
- (map (\<lambda>(n, fs). (n, function_sig'.truncate fs)) (funs r2)) sts2 = Inl fs2 \<Longrightarrow>
-list_all2 (alpha_equiv_statement' (locs' # vsubst')) sts1 sts2 \<Longrightarrow>
-
-alpha_equiv_check_decls sts1 sts2 = Some funcs' \<Longrightarrow>
- list_all2 (alpha_equiv_fun (zip (get_fun_decls sts1) (get_fun_decls sts2) # fsubst))
-     (combine_keep (funs r1)
-       (map (\<lambda>(n, fs). (n, function_sig'.extend fs \<lparr>f_sig_visible = map fst fs1\<rparr>)) fs1))
-     (combine_keep (funs r2)
-       (map (\<lambda>(n, fs). (n, function_sig'.extend fs \<lparr>f_sig_visible = map fst fs2\<rparr>)) fs2))
-
-*)
-
   qed
-
 next
   case XS1 : (ExitStatement x1 locs1 funs1)
 
@@ -3363,21 +2263,13 @@ next
         using XS1 D1 VD1 XS2 D2 VD2 Hinit H1 H2 Hc1 Hc2 
         by(auto simp add: alpha_equiv_results'_def)
 
-      show ?thesis using XS1 D1 VD1 XS2 D2 VD2 Hinit H1 H2 Hc1 Hc2 Hupd None1 None2 Vemp Subst_cons
-          L1v L2v
-          alpha_equiv_locals_v_insert[OF L1v[unfolded Vlens] L2v, of substh substt fsubst']
-        apply(auto simp add: alpha_equiv_results'_def)
-          defer
+      show ?thesis sorry
 
     next
       case (Some a)
       then show ?thesis sorry
     qed
 
-
-      using XS1 D1 VD1 XS2 D2 VD2 Hinit H1 H2 Hc1 Hc2 Hupd
-      apply(cases eo1; cases eo2; auto simp add: alpha_equiv_results'_def)
-(* again, we need a lemma relating updates to alpha-equivalence *)
   next
 
     case (YulVariableDeclarationStatement x3)
